theories/interop/basics_resources.v
@@ -545,6 +545,32 @@ Proof using.
   all: inversion Hstore.
 Qed.
 
+Lemma block_sim_of_auth_strong (ζfreeze : lstore) (χvirt : lloc_map)
+   v b :
+  is_val χvirt ζfreeze v b →
+  lloc_own_auth χvirt -∗
+  lstore_own_auth ζfreeze -∗
+  b ~~ v.
+Proof using.
+  iIntros (H) "Hχ Hζ".
+  iDestruct (lstore_own_auth_get_immut_all with "Hζ") as "#Hζimm".
+  iInduction H as [] "IH" forall "Hζ Hχ"; cbn; try done.
+  1: iExists γ; iSplit; first done.
+  1: by iApply (lloc_own_auth_get_pub with "Hχ").
+  1: iExists γ, lv1, lv2; iSplit; first done; iSplit.
+  3-4: iExists γ, lv; iSplit; first done; iSplit.
+  7: iExists γ; iSplit; first done.
+  8: iExists γ; iSplit; first done.
+  8: by iApply (lloc_own_auth_get_foreign with "Hχ").
+  1,3,5,7:
+    try iApply lstore_own_vblock_I_as_imm;
+    iApply (big_sepM_lookup with "Hζimm"); try done.
+  5: iSplit.
+  1-4: apply lstore_immut_blocks_lookup_immut; done.
+  1,3,4: iApply ("IH" with "Hζ Hχ").
+  iApply ("IH1" with "Hζ Hχ").
+Qed.
+
 Lemma block_sim_arr_of_auth (ζfreeze ζσ ζvirt : lstore) (χvirt : lloc_map) (σMLvirt : store)
    vs bb :
   ζfreeze = ζσ ∪ ζvirt →
@@ -563,18 +589,31 @@ Proof using.
   eapply Forall2_lookup_lr; done.
 Qed.
 
-Lemma block_sim_auth_is_val  (ζfreeze ζσ ζvirt : lstore) (χvirt : lloc_map) (σMLvirt : store)
+Lemma block_sim_arr_of_auth_strong (ζfreeze : lstore) (χvirt : lloc_map)
+   vs bb :
+  Forall2 (is_val χvirt ζfreeze) vs bb →
+  lloc_own_auth χvirt -∗
+  lstore_own_auth ζfreeze -∗
+  bb ~~∗ vs.
+Proof using.
+  iIntros (H) "Hχ Hζ".
+  iApply big_sepL2_forall; iSplit; first (iPureIntro; by eapply Forall2_length).
+  iIntros "%k %v %l %H1 %H2".
+  iApply (block_sim_of_auth_strong with "Hχ Hζ"); try done.
+  eapply Forall2_lookup_lr; done.
+Qed.
+
+Lemma block_sim_auth_is_val_strong  (ζfreeze ζσ ζvirt ζplus : lstore) (χvirt : lloc_map)
    v b :
   ζfreeze = ζσ ∪ ζvirt →
-  is_store_blocks χvirt σMLvirt ζσ →
-  is_store χvirt ζfreeze σMLvirt →
   ζσ ##ₘ ζvirt →
   lloc_own_auth χvirt -∗
-  lstore_own_auth ζvirt -∗
+  lstore_own_auth (ζplus ∪ ζvirt) -∗
+  ([∗ map] γ↦b ∈ ζplus, ghost_map_elem wrapperG_γζvirt γ (DfracOwn 1) b) -∗
   b ~~ v -∗
   ⌜is_val χvirt ζfreeze v b⌝.
 Proof using.
-  iIntros (Hfreeze Hstorebl Hstore Hdis) "Hχ Hζ Hsim".
+  iIntros (Hfreeze Hdis) "Hχ Hζ Hplus Hsim".
   iInduction v as [[x|bo| | |]| | | |] "IH" forall (b); cbn.
   all: try (iPure "Hsim" as Hsim; subst; iPureIntro; try econstructor; done).
   1: {iDestruct "Hsim" as "(%γ & -> & Hsim)".
@@ -585,34 +624,108 @@ Proof using.
        iPureIntro. econstructor. done. }
   1: iDestruct "Hsim" as "(%γ & -> & Hsim)".
   2: iDestruct "Hsim" as "(%γ & %lv1 & %lv2 & -> & Hsim & Hlv1 & Hlv2)";
-     iPoseProof ("IH" with "Hχ Hζ Hlv1") as "%Hr1";
-     iPoseProof ("IH1" with "Hχ Hζ Hlv2") as "%Hr2".
+     iPoseProof ("IH" with "Hχ Hζ Hplus Hlv1") as "%Hr1";
+     iPoseProof ("IH1" with "Hχ Hζ Hplus Hlv2") as "%Hr2".
   3-4: iDestruct "Hsim" as "(%γ & %lv & -> & Hsim & Hlv)";
-       iPoseProof ("IH" with "Hχ Hζ Hlv") as "%Hr".
+       iPoseProof ("IH" with "Hχ Hζ Hplus Hlv") as "%Hr".
   all: try iDestruct (lstore_own_vblock_I_as_imm with "Hsim") as "Hsim".
-  1-4: unshelve iPoseProof (lstore_own_immut_of with "Hζ Hsim") as "[%HH _]".
+  1-4: unshelve iPoseProof (lstore_own_immut_of with "Hζ Hsim") as "#[%HH _]".
+  all: eapply lookup_union_Some_raw in HH as [HH|(Hne&HH)]; last
+       (iDestruct "Hsim" as "(Hsim&_)"; rewrite /lstore_own_immut; try iDestruct "Hsim" as "(Hsim&_)").
+  1: iPoseProof (lstore_own_immut_to_elem with "Hsim") as "Hsim";
+     iPoseProof (big_sepM_lookup_acc with "Hplus") as "(Hcontr&_)"; first done;
+     cbn; iPoseProof (ghost_map_elem_ne with "Hcontr Hsim") as "%HH2"; done.
+  2: iPoseProof (lstore_own_immut_to_elem with "Hsim") as "Hsim";
+     iPoseProof (big_sepM_lookup_acc with "Hplus") as "(Hcontr&_)"; first done;
+     cbn; iPoseProof (ghost_map_elem_ne with "Hcontr Hsim") as "%HH2"; done.
+  3: iPoseProof (lstore_own_immut_to_elem with "Hsim") as "Hsim";
+     iPoseProof (big_sepM_lookup_acc with "Hplus") as "(Hcontr&_)"; first done;
+     cbn; iPoseProof (ghost_map_elem_ne with "Hcontr Hsim") as "%HH2"; done.
+  4: iPoseProof (lstore_own_immut_to_elem with "Hsim") as "Hsim";
+     iPoseProof (big_sepM_lookup_acc with "Hplus") as "(Hcontr&_)"; first done;
+     cbn; iPoseProof (ghost_map_elem_ne with "Hcontr Hsim") as "%HH2"; done.
   all: iPureIntro; econstructor; eauto; by simplify_map_eq.
 Qed.
 
-Lemma block_sim_arr_auth_is_val (ζfreeze ζσ ζvirt : lstore) (χvirt : lloc_map) (σMLvirt : store)
+Lemma block_sim_auth_is_val  (ζfreeze ζσ ζvirt : lstore) (χvirt : lloc_map)
+   v b :
+  ζfreeze = ζσ ∪ ζvirt →
+  ζσ ##ₘ ζvirt →
+  lloc_own_auth χvirt -∗
+  lstore_own_auth ζvirt -∗
+  b ~~ v -∗
+  ⌜is_val χvirt ζfreeze v b⌝.
+Proof using.
+  iIntros (Hfreeze Hdis) "Hχ Hζ Hsim".
+  iApply (block_sim_auth_is_val_strong _ _ _ ∅ with "Hχ [Hζ] [] Hsim").
+  - apply Hfreeze.
+  - apply Hdis.
+  - by rewrite map_empty_union.
+  - done.
+Qed.
+
+Lemma block_sim_auth_is_val_simple (ζfreeze : lstore) (χvirt : lloc_map)
+   v b :
+  lloc_own_auth χvirt -∗
+  lstore_own_auth ζfreeze -∗
+  b ~~ v -∗
+  ⌜is_val χvirt ζfreeze v b⌝.
+Proof using.
+  iIntros "Hχ Hζ Hsim".
+  iApply (block_sim_auth_is_val _ ∅ _ with "Hχ Hζ Hsim").
+  - by rewrite map_empty_union.
+  - eapply map_disjoint_empty_l.
+Qed.
+
+Lemma block_sim_arr_auth_is_val_strong (ζfreeze ζσ ζvirt ζplus : lstore) (χvirt : lloc_map)
    vs bb :
   ζfreeze = ζσ ∪ ζvirt →
-  is_store_blocks χvirt σMLvirt ζσ →
-  is_store χvirt ζfreeze σMLvirt →
+  ζσ ##ₘ ζvirt →
+  lloc_own_auth χvirt -∗
+  lstore_own_auth (ζplus ∪ ζvirt) -∗
+  ([∗ map] γ↦b ∈ ζplus, ghost_map_elem wrapperG_γζvirt γ (DfracOwn 1) b) -∗
+  bb ~~∗ vs -∗
+  ⌜Forall2 (is_val χvirt ζfreeze) vs bb⌝.
+Proof using.
+  iIntros (Hfreeze Hdis) "Hχ Hζ Hplus Hsim".
+  iPoseProof (big_sepL2_forall with "Hsim") as "(%Heq & Hsim)".
+  iAssert (⌜(∀ i x y, vs !! i = Some x → bb !! i = Some y → is_val χvirt ζfreeze x y)⌝)%I as "%HF".
+  2: iPureIntro; by apply Forall2_same_length_lookup_2.
+  iIntros (i v b H1 H2).
+  iApply (block_sim_auth_is_val_strong with "Hχ Hζ Hplus"); try done.
+  iApply ("Hsim" $! i v b H1 H2).
+Qed.
+
+Lemma block_sim_arr_auth_is_val (ζfreeze ζσ ζvirt : lstore) (χvirt : lloc_map)
+   vs bb :
+  ζfreeze = ζσ ∪ ζvirt →
   ζσ ##ₘ ζvirt →
   lloc_own_auth χvirt -∗
   lstore_own_auth ζvirt -∗
   bb ~~∗ vs -∗
   ⌜Forall2 (is_val χvirt ζfreeze) vs bb⌝.
 Proof using.
-  iIntros (Hfreeze Hstorebl Hstore Hdis) "Hχ Hζ Hsim".
-  iPoseProof (big_sepL2_forall with "Hsim") as "(%Heq & Hsim)".
-  iAssert (⌜(∀ i x y, vs !! i = Some x → bb !! i = Some y → is_val χvirt ζfreeze x y)⌝)%I as "%HF".
-  2: iPureIntro; by apply Forall2_same_length_lookup_2.
-  iIntros (i v b H1 H2).
-  iApply (block_sim_auth_is_val with "Hχ Hζ"); try done.
-  iApply ("Hsim" $! i v b H1 H2).
+  iIntros (Hfreeze Hdis) "Hχ Hζ Hsim".
+  iApply (block_sim_arr_auth_is_val_strong _ _ _ ∅ with "Hχ [Hζ] [] Hsim").
+  - apply Hfreeze.
+  - apply Hdis.
+  - by rewrite map_empty_union.
+  - done.
 Qed.
+
+Lemma block_sim_arr_auth_is_val_simple (ζfreeze : lstore) (χvirt : lloc_map)
+   vs bb :
+  lloc_own_auth χvirt -∗
+  lstore_own_auth ζfreeze -∗
+  bb ~~∗ vs -∗
+  ⌜Forall2 (is_val χvirt ζfreeze) vs bb⌝.
+Proof using.
+  iIntros "Hχ Hζ Hsim".
+  iApply (block_sim_arr_auth_is_val _ ∅ _ with "Hχ Hζ Hsim").
+  - by rewrite map_empty_union.
+  - eapply map_disjoint_empty_l.
+Qed.
+
 
 End BasicsResources.
 
