theories/interop/update_laws.v
@@ -2,7 +2,7 @@ From Coq Require Import ssreflect.
 From stdpp Require Import gmap.
 From transfinite.base_logic.lib Require Import ghost_map ghost_var.
 From iris.proofmode Require Import proofmode.
-From melocoton Require Import named_props.
+From melocoton Require Import named_props stdpp_extra.
 From melocoton.c_interface Require Import defs resources.
 From melocoton.ml_lang Require Import lang primitive_laws.
 From melocoton.interop Require Import basics basics_resources gctoken.
@@ -15,49 +15,123 @@ Context `{!heapG_ML Σ, !heapG_C Σ}.
 Context `{!invG Σ}.
 Context `{!wrapperGCtokG Σ}.
 
+
+Lemma foo_lloc_map_inj χ : lloc_map_inj χ → gmap_inj (lloc_map_pubs χ).
+Proof.
+  intros H γ1 γ2 ℓ H1%lloc_map_pubs_lookup_Some H2%lloc_map_pubs_lookup_Some.
+  eapply H. all: done.
+Qed.
+
+Lemma GC_per_loc_modify_σ M ζ σMLvirt γ ℓ' v:
+  gmap_inj M →
+  M !! γ = Some ℓ' →
+(([∗ map] ℓ↦y ∈ delete γ M, per_location_invariant ζ σMLvirt ℓ y)
+⊢ [∗ map] ℓ↦y ∈ delete γ M, per_location_invariant ζ (<[ ℓ' := v ]> σMLvirt) ℓ y)%I.
+Proof.
+  iIntros (Hinj Hlu) "Hbig".
+  iApply (big_sepM_wand with "Hbig").
+  iApply (big_sepM_intro).
+  iIntros "!>" (γ2 ℓ (Hne&Hlu2)%lookup_delete_Some) "(%vs'&%tg&%lvs&[(Hℓ&#Hsim)|[(%Hℓσ&Hγ&#Hsim)|[(%Hnone1&%Hnone2)|(%Hnone1&%Hnone2)]]])"; iExists vs', tg, lvs.
+  - iLeft; by iFrame.
+  - iRight. iLeft. iFrame "Hγ Hsim". iPureIntro.
+    rewrite lookup_insert_ne; first done.
+    intros ->. by eapply Hne, Hinj.
+  - iRight. iRight. iLeft. iPureIntro. split; last done.
+    rewrite lookup_insert_ne; try done.
+    intros ->. by eapply Hne, Hinj.
+  - iRight. iRight. iRight. iFrame. iPureIntro; split; last done.
+    rewrite lookup_insert_ne; first done.
+    intros ->. by eapply Hne, Hinj.
+Qed.
+
+Lemma GC_per_loc_insert M ζ σMLvirt ℓ' v:
+  (∀ γ, M !! γ ≠ Some ℓ') →
+(([∗ map] γ↦ℓ ∈ M, per_location_invariant ζ σMLvirt γ ℓ)
+⊢ [∗ map] γ↦ℓ ∈ M, per_location_invariant ζ (<[ ℓ' := v ]> σMLvirt) γ ℓ)%I.
+Proof.
+  iIntros (Hnℓ) "Hbig".
+  iApply (big_sepM_wand with "Hbig").
+  iApply (big_sepM_intro).
+  iIntros "!>" (γ2 ℓ Hne) "(%vs'&%tg&%lvs&[(Hℓ&#Hsim)|[(%Hℓσ&Hγ&#Hsim)|[(%Hnone1&%Hnone2)|(%Hnone1&%Hnone2)]]])"; iExists vs', tg, lvs.
+  - iLeft; by iFrame.
+  - iRight. iLeft. iFrame "Hγ Hsim". iPureIntro.
+    rewrite lookup_insert_ne; first done.
+    intros ->. eapply Hnℓ, Hne.
+  - iRight. iRight. iLeft. iSplit; last done. iPureIntro.
+    rewrite lookup_insert_ne; try done.
+    intros ->. eapply Hnℓ, Hne.
+  - do 3 iRight. iFrame. iPureIntro; split; last done.
+    rewrite lookup_insert_ne; first done.
+    intros ->. by eapply Hnℓ, Hne.
+Qed.
+
+Lemma GC_per_loc_modify_ζ M ζ σMLvirt γ v:
+  M !! γ = None →
+(([∗ map] ℓ↦y ∈ M, per_location_invariant ζ σMLvirt ℓ y)
+⊢ [∗ map] ℓ↦y ∈ M, per_location_invariant (<[ γ := v ]> ζ) σMLvirt ℓ y)%I.
+Proof.
+  iIntros (Hne) "Hbig".
+  iApply (big_sepM_wand with "Hbig").
+  iApply (big_sepM_intro).
+  iIntros "!>" (γ2 ℓ Hle) "(%vs'&%tg&%lvs&[(Hℓ&#Hsim)|[(%Hℓσ&Hγ&Hsim&%Heq)|[(%Hnone1&%Hnone2)|(Hnone1&%Hnone2)]]])"; iExists vs', tg, lvs.
+  - iLeft. iFrame. rewrite lookup_insert_ne; first done.
+    intros ->; congruence.
+  - iRight. iLeft. by iFrame.
+  - iRight. iRight. iLeft. iPureIntro; split; first done.
+    rewrite lookup_insert_ne; try done.
+    intros ->. simplify_eq.
+  - do 3 iRight. iFrame. iPureIntro.
+    rewrite lookup_insert_ne; try done.
+    intros ->. simplify_eq.
+Qed.
+
+Lemma GC_per_loc_delete_ζ M ζ σMLvirt γ:
+  M !! γ = None →
+(([∗ map] ℓ↦y ∈ M, per_location_invariant ζ σMLvirt ℓ y)
+⊢ [∗ map] ℓ↦y ∈ M, per_location_invariant (delete γ ζ) σMLvirt ℓ y)%I.
+Proof.
+  iIntros (Hne) "Hbig".
+  iApply (big_sepM_wand with "Hbig").
+  iApply (big_sepM_intro).
+  iIntros "!>" (γ2 ℓ Hle) "(%vs'&%tg&%lvs&[(Hℓ&#Hsim)|[(%Hℓσ&Hγ&Hsim&%Heq)|[(%Hnone1&%Hnone2)|(Hnone1&%Hnone2)]]])"; iExists vs', tg, lvs.
+  - iLeft. iFrame. rewrite lookup_delete_ne; first done.
+    intros ->; congruence.
+  - iRight. iLeft. by iFrame.
+  - iRight. iRight. iLeft. iPureIntro; split; first done.
+    rewrite lookup_delete_ne; try done.
+    intros ->. simplify_eq.
+  - do 3 iRight. iFrame. iPureIntro. apply lookup_delete_None; by right.
+Qed.
+
 Lemma ml_to_mut θ ℓ vs :
   ⊢ GC θ ∗ ℓ ↦∗ vs ==∗
     GC θ ∗ ∃ lvs γ, γ ↦mut (TagDefault, lvs) ∗ γ ~ℓ~ ℓ ∗ lvs ~~∗ vs.
 Proof using.
-  iIntros "(HGC & Hl)". iNamed "HGC".
+  iIntros "(HGC & Hl)". iNamed "HGC". iNamed "HSI_block_level".
   iDestruct (gen_heap_valid with "GCσMLv Hl") as %Hlσ.
-  edestruct is_store_blocks_has_loc as (ll & Hlχ & Hllζ);
-    [apply Hstore_blocks|apply Hlσ|..].
+  destruct (Hstore ℓ) as (γ & Hχγ%lloc_map_pubs_lookup_Some); first by eapply elem_of_dom_2.
+  iPoseProof (big_sepM_delete _ _ _ _ Hχγ with "GC_per_loc") as "((%vs'&%tg&%lvs&[(Hℓ&_)|[(%Hℓσ&Hγ&#Hsim&->)|[(%Hne1&%Hne2)|(%Hne1&%Hne2)]]])&GC_per_loc)".
+  1: by iPoseProof (gen_heap.mapsto_ne with "Hl Hℓ") as "%Hbot".
+  2: by simplify_eq.
+  2: by simplify_eq.
+  simplify_eq.
   iMod (gen_heap_update _ _ _ None with "GCσMLv Hl") as "[GCσMLv Hl]".
-  apply elem_of_dom in Hllζ. destruct Hllζ as [bb Hζσll].
-  assert (ζfreeze !! ll = Some bb) as Hfreezell.
-  1: { rewrite Hfreezeeq. by apply lookup_union_Some_l. }
-  unfold is_store in Hstore.
-  specialize (Hstore ℓ vs ll bb Hlσ Hlχ Hfreezell) as Hstorel.
-  inversion Hstorel; subst vs0 bb.
-  iAssert (block_sim_arr vs lvs) as "#Hblock".
-  1: by iApply (block_sim_arr_of_auth with "GCχvirt GCζvirt").
-  iAssert (ll ~ℓ~ ℓ) as "#Hraw".
-  1: by iApply (lloc_own_auth_get_pub with "GCχvirt").
-  iMod (lstore_own_insert _ ll (Bvblock (Mut, _)) with "GCζvirt") as "(GCζvirt & Hzz)".
-  1: { eapply map_disjoint_Some_l; done. }
-  iDestruct (lstore_own_elem_to_mut with "Hzz") as "Hzz"; first done.
+  iDestruct "Hγ" as "(Hγ1&(%ℓ'&#Hγ2))".
+  iPoseProof (lstore_own_elem_of with "GCζauth Hγ1") as "%Hγζ".
+  iPoseProof (GC_per_loc_modify_σ with "GC_per_loc") as "GC_per_loc".
+  1: by eapply foo_lloc_map_inj, expose_llocs_inj. 1: done.
+  iPoseProof (big_sepM_delete _ _ _ _ Hχγ with "[$GC_per_loc Hl]") as "GC_per_loc".
+  { iExists vs, TagDefault, lvs. iLeft. by iFrame. }
+  iPoseProof (lloc_own_pub_of with "GCχauth Hγ2") as "%Hγℓ".
+  apply lloc_map_pubs_lookup_Some in Hγℓ; simplify_eq.
   iModIntro.
-  assert (ζvirt !! ll = None) as HζllNone.
-  1: eapply map_disjoint_Some_l; done.
-  iSplitR "Hzz".
-  { rewrite /GC /named.
-    iExists ζ, ζfreeze, (delete ll ζσ), (<[ll:=(Bvblock (Mut, (TagDefault, lvs)))]> ζvirt).
-    iExists χ, χvirt, (<[ℓ:=None]> σMLvirt), roots_s, roots_m. iFrame.
-    iSplit.
-    { rewrite (pub_locs_in_lstore_insert_lstore_pub _ _ _ ℓ) //.
-      iApply big_sepM_insert; eauto. by iFrame. }
-    iPureIntro. split_and!; eauto.
-    - symmetry. subst. by apply union_delete_insert.
-    - apply map_disjoint_insert_r_2. 1: apply lookup_delete.
-      apply map_disjoint_delete_l. done.
-    - eapply is_store_blocks_discard_loc; eauto.
-    - intros γ [bl [[<-  <- ]|[? ?]]%lookup_insert_Some]%elem_of_dom.
-      1: by eapply elem_of_dom_2.
-      apply Hother_blocks; by eapply elem_of_dom_2.
-    - eapply is_store_discard_loc; eauto. }
-  { iExists lvs, ll. iFrame "Hraw Hblock ∗".
-    iApply lstore_own_vblock_M_as_mut; eauto. }
+  iSplitR "Hγ1".
+  2: iExists _, _; iFrame; iFrame "Hsim Hγ2"; by iExists _.
+  rewrite /GC /SI_block_level /named.
+  iExists ζ, ζ_future, χ, χ_future, roots_s. iFrame "GCζ GCχ GCθ GCroots GCinit GCχauth HSI_GC". iSplit; last done.
+  iExists (<[ℓ:=None]> σMLvirt). iFrame.
+  iPureIntro. split_and!; try done.
+  by rewrite dom_insert_lookup_L.
 Qed.
 
 Lemma mut_to_ml γ vs lvs θ :
@@ -66,34 +140,29 @@ Lemma mut_to_ml γ vs lvs θ :
 Proof using.
   iIntros "(HGC & Hl & #Hsim)".
   iDestruct (lstore_own_vblock_M_as_mut with "Hl") as "(Hl & (%ℓ & #Hlℓ))".
-  iNamed "HGC".
-  iDestruct (block_sim_arr_auth_is_val with "GCχvirt GCζvirt Hsim") as %Hsim;
-    try done.
-  iPoseProof (lloc_own_pub_of with "GCχvirt Hlℓ") as "%Hχℓ".
-  unfold is_store in Hstore.
-  iDestruct (lstore_own_mut_of with "GCζvirt Hl") as %[Hζl _].
-  iDestruct (big_sepM_delete _ _ _ ℓ with "GCχNone") as "[Hℓ GCχNone]".
-  { eapply map_filter_lookup_Some. rewrite lloc_map_pubs_lookup_Some.
-    split; eauto. by eapply elem_of_dom_2. }
-  iDestruct (gen_heap_valid with "GCσMLv Hℓ") as "%Hlσ".
+  iNamed "HGC". iNamed "HSI_block_level".
+  iPoseProof (lstore_own_mut_of with "GCζauth Hl") as "(%Hγζ&#_)".
+  iPoseProof (lloc_own_pub_of with "GCχauth Hlℓ") as "%Hχγ".
+  apply lloc_map_pubs_lookup_Some in Hχγ.
+  iPoseProof (big_sepM_delete _ _ _ _ Hχγ with "GC_per_loc") as "((%vs'&%tg&%lvs'&[(Hℓ&%Hγζ')|[(%Hℓσ&(Hγ&_)&_)|[(%Hne1&%Hne2)|(Hne1&%Hne2)]]])&GC_per_loc)".
+  2: iDestruct "Hl" as "(Hl&_)"; by iPoseProof (ghost_map_elem_ne with "Hl Hγ") as "%Hne".
+  2: simplify_eq.
+  2: simplify_eq.
+  iDestruct (gen_heap_valid with "GCσMLv Hℓ") as %Hℓσ.
   iMod (gen_heap_update _ _ _ (Some vs) with "GCσMLv Hℓ") as "[GCσMLv Hℓ]".
-  iMod (lstore_own_delete with "GCζvirt Hl") as "GCζvirt".
-  iModIntro. iSplitR "Hℓ".
-  { rewrite /GC /named.
-    iExists ζ, ζfreeze, (<[γ:=(Bvblock (Mut, (TagDefault, lvs)))]> ζσ), (delete γ ζvirt).
-    iExists χ, χvirt, (<[ℓ := Some vs]> σMLvirt), roots_s, roots_m. iFrame.
-    iSplit; first by rewrite pub_locs_in_lstore_delete_lstore //.
-    iPureIntro; split_and!; eauto.
-  + erewrite (union_insert_delete ζσ ζvirt). 2: eapply map_disjoint_Some_r. all: eauto.
-  + apply map_disjoint_insert_l_2. 1: apply lookup_delete.
-    apply map_disjoint_delete_r. done.
-  + eapply is_store_blocks_restore_loc; eauto.
-  + intros γ' [blk [Hne Hblk]%lookup_delete_Some]%elem_of_dom. eapply Hother_blocks.
-    by eapply elem_of_dom_2.
-  + eapply is_store_restore_loc; eauto.
-    { rewrite Hfreezeeq. eapply lookup_union_Some_r; eauto. }
-    by constructor. }
-  { iExists _. eauto. }
+  iPoseProof (GC_per_loc_modify_σ with "GC_per_loc") as "GC_per_loc".
+  1: by eapply foo_lloc_map_inj, expose_llocs_inj. 1: done.
+  iPoseProof (big_sepM_delete _ _ _ _ Hχγ with "[$GC_per_loc Hl]") as "GC_per_loc".
+  { iExists vs, TagDefault, lvs. iRight; iLeft. rewrite lookup_insert. repeat iSplit; try done.
+    1: by iApply lstore_own_mut_to_elem. by iExists _. }
+  iModIntro.
+  iSplitR "Hℓ".
+  2: iExists _; iFrame "Hℓ Hlℓ".
+  rewrite /GC /SI_block_level /named.
+  iExists ζ, ζ_future, χ, χ_future, roots_s. iFrame. iSplit; last done.
+  iExists (<[ℓ:=_]> σMLvirt). iFrame.
+  iPureIntro. split_and!; try done.
+  by rewrite dom_insert_lookup_L.
 Qed.
 
 Lemma freeze_to_mut γ lvs θ :
@@ -102,35 +171,40 @@ Lemma freeze_to_mut γ lvs θ :
 Proof using.
   iIntros "(HGC & Hγ)".
   iDestruct (lstore_own_vblock_F_as_mut with "Hγ") as "(Hmtζ & Hmtfresh)".
-  iNamed "HGC".
-  iDestruct (lstore_own_mut_of with "GCζvirt Hmtζ") as %[Hζγ _].
-  pose (fresh_locs (lloc_map_pub_locs χvirt)) as ℓ.
-  assert (ℓ ∉ lloc_map_pub_locs χvirt).
-  { intros Hℓ. apply (fresh_locs_fresh (lloc_map_pub_locs χvirt) 0 ltac:(lia)).
+  iNamed "HGC". iNamed "HSI_block_level".
+  iDestruct (lstore_own_mut_of with "GCζauth Hmtζ") as %[Hζγ _].
+  pose (fresh_locs (lloc_map_pub_locs χ_future)) as ℓ.
+  assert (ℓ ∉ lloc_map_pub_locs χ_future).
+  { intros Hℓ. apply (fresh_locs_fresh (lloc_map_pub_locs χ_future) 0 ltac:(lia)).
     rewrite /loc_add Z.add_0_r //. }
   assert (ℓ ∉ dom σMLvirt).
-  { intros Hℓ. destruct Hstore_blocks as [H1 _].
-    destruct (H1 _ Hℓ) as (γ'&Hγ'). by apply elem_of_lloc_map_pub_locs_1 in Hγ'. }
-  iDestruct (lloc_own_priv_of with "GCχvirt Hmtfresh") as %Hχvirtγ.
-  iMod (lloc_own_expose with "GCχvirt Hmtfresh") as "[GCχvirt #Hℓγ]".
+  { intros Hℓ.
+    destruct (Hstore _ Hℓ) as (γ'&Hγ'). by apply elem_of_lloc_map_pub_locs_1 in Hγ'. }
+  iDestruct (lloc_own_priv_of with "GCχauth Hmtfresh") as %Hχγ.
+  iMod (lloc_own_expose _ _ ℓ with "GCχauth Hmtfresh") as "[GCχvirt #Hℓγ]".
   iMod (gen_heap_alloc _ ℓ None with "GCσMLv") as "(GCσMLv & HℓNone & Hmeta)".
   1: by eapply not_elem_of_dom_1.
-  iPoseProof (big_sepM_insert _ _ γ ℓ with "[$GCχNone $HℓNone]") as "GCχNone".
-  { eapply map_filter_lookup_None. left. eapply lloc_map_pubs_lookup_None; eauto. }
+  destruct lvs as [tg lvs].
+  iPoseProof (GC_per_loc_insert _ _ _ ℓ with "GC_per_loc") as "GC_per_loc".
+  1: { intros γ' Hγ'%lloc_map_pubs_lookup_Some. apply elem_of_lloc_map_pub_locs_1 in Hγ'. apply H, Hγ'. }
+  iPoseProof (big_sepM_insert _ _ γ ℓ with "[$GC_per_loc HℓNone]") as "GC_per_loc".
+  1: eapply lloc_map_pubs_lookup_None; eauto.
+  1: iExists nil, tg, lvs; iLeft; by iFrame.
   iModIntro. iSplitR "Hℓγ Hmtζ".
   2: { iApply lstore_own_vblock_M_as_mut. iFrame "Hmtζ". eauto. }
-  rewrite /GC /named.
-  iExists ζ, ζfreeze, ζσ, ζvirt.
-  iExists χ, (<[γ:=LlocPublic ℓ]> χvirt), (<[ℓ:=None]> σMLvirt), roots_s, roots_m.
-  iFrame. iSplit.
-  { rewrite pub_locs_in_lstore_insert_pub //. by eapply elem_of_dom_2. }
-  iPureIntro; split_and!; eauto.
-  + eapply is_store_blocks_expose_lloc; eauto.
-  + intros γ' Hγ'. rewrite dom_insert_L. eapply elem_of_union; right.
-    by apply Hother_blocks.
-  + eapply is_store_expose_lloc; eauto.
-  + eapply expose_llocs_trans; first eassumption.
-    eapply expose_llocs_insert; eauto.
+  rewrite /GC /SI_block_level /named.
+  iExists ζ, ζ_future, χ, (<[γ:=LlocPublic ℓ]> χ_future), roots_s.
+  iFrame "GCζ GCχ GCθ GCroots GCinit GCχvirt HSI_GC". iSplit; last first.
+  { iSplit; first done.
+    iPureIntro. eapply expose_llocs_trans; first eassumption.
+    eapply expose_llocs_insert; eauto. }
+  iExists (<[ℓ:=None]> σMLvirt). rewrite lloc_map_pubs_insert_pub.
+  iFrame. iPureIntro; split_and!; eauto.
+  + rewrite dom_insert. set_solver.
+  + intros ℓ'. rewrite !dom_insert_L elem_of_union elem_of_singleton.
+    intros [<-|Hℓ']. 1: by exists γ; simplify_map_eq.
+    specialize (Hstore _ Hℓ') as (γ'&?). exists γ'.
+    rewrite lookup_insert_ne //. set_solver.
 Qed.
 
 Lemma freeze_to_immut γ lvs θ :
@@ -139,29 +213,26 @@ Lemma freeze_to_immut γ lvs θ :
 Proof using.
   iIntros "(HGC & Hγ)".
   iDestruct (lstore_own_vblock_F_as_mut with "Hγ") as "(Hmtζ & Hmtfresh)".
-  iNamed "HGC".
-  iDestruct (lstore_own_mut_of with "GCζvirt Hmtζ") as %[Hζγ _].
-  iDestruct (lloc_own_priv_of with "GCχvirt Hmtfresh") as %Hχvirtγ.
-  iMod (lstore_own_update _ _ _ (Bvblock (Immut, lvs)) with "GCζvirt Hmtζ") as "(GCζvirt & Hmtζ)".
+  iNamed "HGC". iNamed "HSI_block_level". iNamed "HSI_GC".
+  iDestruct (lstore_own_mut_of with "GCζauth Hmtζ") as %[Hζγ _].
+  iDestruct (lloc_own_priv_of with "GCχauth Hmtfresh") as %Hχγ.
+  iMod (lstore_own_update _ _ _ (Bvblock (Immut, lvs)) with "GCζauth Hmtζ") as "(GCζauth & Hmtζ)".
   iDestruct (lstore_own_elem_to_immut with "Hmtζ") as "Hmtζ"; first done.
+  iPoseProof (GC_per_loc_modify_ζ with "GC_per_loc") as "GC_per_loc".
+  1: eapply lloc_map_pubs_lookup_None; right; left; eapply Hχγ.
   iModIntro.
   iSplitR "Hmtζ"; last by iApply lstore_own_vblock_I_as_imm.
-  rewrite /GC /named.
-  iExists ζ, (<[γ:=(Bvblock (Immut, lvs))]> ζfreeze), ζσ, (<[γ:=(Bvblock (Immut, lvs))]> ζvirt).
-  iExists χ, χvirt, σMLvirt, roots_s, roots_m. iFrame.
-  assert (Hζγ': ζfreeze !! γ = Some (Bvblock (Mut, lvs))).
-  { subst. rewrite lookup_union_r; eauto. by eapply map_disjoint_Some_l. }
+  rewrite /GC /SI_block_level /SI_GC /named.
+  iExists ζ, (<[γ:=(Bvblock (Immut, lvs))]> ζ_future), χ, χ_future, roots_s.
+  iFrame "GCζ GCχ GCθ GCroots GCinit GCχauth GCζauth".
+  iSplitL "GCσMLv GC_per_loc".
+  { iExists σMLvirt.
+    iFrame; iPureIntro; split_and!; eauto. by rewrite dom_insert_lookup_L. }
   iSplit.
-  { rewrite pub_locs_in_lstore_insert_existing; eauto. by eapply elem_of_dom_2. }
-  iPureIntro; split_and!; eauto.
-  + eapply freeze_lstore_freeze_lloc; eauto.
-  + subst. rewrite insert_union_r. 1: done. eapply map_disjoint_Some_l; done.
-  + apply map_disjoint_insert_r. split; last done. by eapply map_disjoint_Some_l.
-  + intros γ' [bl [[<-  <- ]|[? ?]]%lookup_insert_Some]%elem_of_dom.
-      1: by eapply elem_of_dom_2.
-      apply Hother_blocks; by eapply elem_of_dom_2.
-  + eapply is_store_freeze_lloc; eauto.
-  + eapply GC_correct_freeze_lloc; eauto.
+  { iExists roots_m. iFrame. iPureIntro; split_and!; eauto.
+    eapply GC_correct_freeze_lloc; eauto. }
+  iPureIntro; split_and; eauto.
+  eapply freeze_lstore_freeze_lloc; eauto.
 Qed.
 
 Lemma update_root θ (l:loc) v E :
@@ -170,17 +241,18 @@ Lemma update_root θ (l:loc) v E :
     (∀ v' w', l ↦C w' ∗ ⌜repr_lval θ v' w'⌝ ={E}=∗ GC θ ∗ l ↦roots v').
 Proof using.
   iIntros "(HGC & Hroots)".
-  iNamed "HGC".
+  iNamed "HGC". iNamed "HSI_GC".
   iPoseProof (ghost_map_lookup with "GCrootsm Hroots") as "%H".
   iPoseProof (big_sepM_delete) as "(HL&_)"; first apply H.
   iPoseProof ("HL" with "GCrootspto") as "((%w&Hown&%Hrepr2) & Hrp)"; iClear "HL".
   iExists _. iFrame "Hown". iSplit; first done. iIntros (v' w') "(Hown' & %Hrepr')".
   iMod (ghost_map_update with "GCrootsm Hroots") as "(GCrootsm&Hroots)".
-  iModIntro. iFrame "Hroots". do 9 iExists _; rewrite /named. iFrame.
-  rewrite dom_insert_lookup_L; last done.
+  iModIntro. iFrame "Hroots". do 5 iExists _. iFrame.
+  iSplit; last done.
+  rewrite /SI_GC /named. iExists _. iFrame. rewrite dom_insert_lookup_L; last done.
   iSplit.
-  { iPoseProof (big_sepM_insert_delete) as "(_&HR)"; iApply "HR"; iClear "HR".
-    iFrame. iExists _. by iFrame. }
+  { iPoseProof (big_sepM_insert_delete) as "(_&HR)"; iApply "HR"; iClear "HR";
+    iFrame; iExists _; by iFrame. }
   { iPureIntro; split_and!; eauto.
     intros l' γ [[-> ->]|[Hne HH]]%lookup_insert_Some.
     2: by eapply Hrootslive.
@@ -192,12 +264,16 @@ Lemma access_root θ (l:loc) dq v :
   ∃ w, l ↦C w ∗ ⌜repr_lval θ v w⌝ ∗
       (l ↦C w -∗ GC θ ∗ l ↦roots{dq} v).
 Proof using.
-  iIntros "(HGC & Hroot)". iNamed "HGC".
+  iIntros "(HGC & Hroot)".
+  iNamed "HGC". iNamed "HSI_GC".
   iPoseProof (ghost_map_lookup with "GCrootsm Hroot") as "%H".
   iPoseProof (big_sepM_delete) as "(HL&HR)"; first apply H.
   iPoseProof ("HL" with "GCrootspto") as "((%w&Hown&%Hrepr2) & Hrp)"; iClear "HL".
   iExists _. iFrame "Hown". iSplit; first done. iIntros "Hown". iFrame "Hroot".
-  rewrite /GC /named. do 9 iExists _.
+  do 5 iExists _. iFrame.
+  iSplit; last done.
+  rewrite /SI_GC /named. iExists _. iFrame "GCrootsm".
+  rewrite /GC /named.
   iPoseProof ("HR" with "[Hown Hrp]") as "Hrootsm"; iClear "HR".
   { iFrame. iExists w; by iFrame. }
   iFrame. eauto.
@@ -209,14 +285,15 @@ Lemma lloc_own_pub_inj θ γ1 γ2 ℓ1 ℓ2 :
  -∗ GC θ
  -∗ GC θ ∗ ⌜γ1 = γ2 ↔ ℓ1 = ℓ2⌝.
 Proof.
-  iIntros "#Hsim1 #Hsim2 HGC". iNamed "HGC".
+  iIntros "#Hsim1 #Hsim2 HGC". iNamed "HGC". iNamed "HSI_block_level".
   iPoseProof (lloc_own_pub_of with "[$] Hsim1") as "%HH1".
   iPoseProof (lloc_own_pub_of with "[$] Hsim2") as "%HH2".
   iSplit.
-  1: (repeat iExists _; iFrame; done).
+  1: (repeat iExists _; iFrame; try done; iSplit; first repeat iExists _; iFrame; done).
   iPureIntro; split; intros ->.
   - by simplify_eq.
-  - destruct Hχvirt as [_ [H _]]. by eapply H.
+  - apply expose_llocs_inj in Hχfuture.
+    by eapply Hχfuture.
 Qed.
 
 Lemma lloc_own_foreign_inj θ γ1 γ2 fid1 fid2 :
@@ -225,14 +302,14 @@ Lemma lloc_own_foreign_inj θ γ1 γ2 fid1 fid2 :
  -∗ GC θ
  -∗ GC θ ∗ ⌜γ1 = γ2 ↔ fid1 = fid2⌝.
 Proof.
-  iIntros "#Hsim1 #Hsim2 HGC". iNamed "HGC".
+  iIntros "#Hsim1 #Hsim2 HGC". iNamed "HGC". iNamed "HSI_block_level".
   iPoseProof (lloc_own_foreign_of with "[$] Hsim1") as "%HH1".
   iPoseProof (lloc_own_foreign_of with "[$] Hsim2") as "%HH2".
   iSplit.
-  1: (repeat iExists _; iFrame; done).
+  1: (repeat iExists _; iFrame; try done; iSplit; first repeat iExists _; iFrame; done).
   iPureIntro; split; intros ->.
   - by simplify_eq.
-  - destruct Hχvirt as [_ [H _]]. by eapply H.
+  - destruct Hχfuture as [_ [H _]]. by eapply H.
 Qed.
 
 
