theories/interop/wp_boundary_laws.v
@@ -9,7 +9,7 @@ From transfinite.base_logic.lib Require Import ghost_map ghost_var.
 From iris.proofmode Require Import proofmode.
 From melocoton.c_interface Require Import defs resources.
 From melocoton.ml_lang Require Import lang lang_instantiation primitive_laws.
-From melocoton.interop Require Import weakestpre wp_utils.
+From melocoton.interop Require Import weakestpre wp_utils update_laws.
 Import Wrap.
 
 (** lemmas to switch between the ML<->C state interp at a boundary *)
@@ -22,6 +22,212 @@ Context `{!heapG_ML Σ, !heapG_C Σ}.
 Context `{!invG Σ}.
 Context `{!wrapperG Σ}.
 
+Lemma GC_SI_to_C σMLvirt ζ ζplus χ :
+    lloc_own_auth χ
+  ∗ lstore_own_auth (ζplus ∪ ζ)
+  ∗ ([∗ map] γ↦b ∈ ζplus, ghost_map_elem wrapperG_γζvirt γ (DfracOwn 1) b)
+  ∗ state_interp (σMLvirt : language.language.state ML_lang)
+  ∗ ([∗ map] γ↦ℓ ∈ lloc_map_pubs χ, per_location_invariant ζ σMLvirt γ ℓ)
+  ∗ ⌜∀ ℓ, ℓ ∈ dom σMLvirt → ∃ γ, χ !! γ = Some (LlocPublic ℓ)⌝
+ ⊢ ∃ ζσ ζvirt,
+    lloc_own_auth χ
+  ∗ lstore_own_auth (ζplus ∪ ζ)
+  ∗ ([∗ map] γ↦b ∈ (ζplus ∪ ζσ), ghost_map_elem wrapperG_γζvirt γ (DfracOwn 1) b)
+  ∗ ([∗ map] γ↦ℓ ∈ lloc_map_pubs χ, per_location_invariant_ML ζvirt γ ℓ)
+  ∗ ⌜ζ = ζσ ∪ ζvirt⌝ ∗ ⌜ζσ ##ₘ ζvirt⌝
+  ∗ state_interp (σMLvirt : language.language.state ML_lang)
+  ∗ ⌜is_store_blocks χ σMLvirt ζσ⌝
+  ∗ ⌜is_store χ ζ σMLvirt⌝.
+Proof.
+  iIntros "(GCχauth&Hplus&GCζauth&GCσMLv&GC_per_loc&%Hstore)".
+  assert (∃ χind, χind ⊆ χ ∧ χ = χind) as (χind&Hsub&Heq).
+  1: eexists _; split; last done; done.
+  rewrite /is_store /is_store_blocks. rewrite {2 4 6 7} Heq.
+  iStopProof. clear Heq. revert ζ ζplus Hsub.
+  induction χind as [|γ [ℓ|fid|] χind Hnone IH] using map_ind;
+  iIntros (ζ ζplus Hsub) "(GCχauth&GCζauth&Hplus&GCσMLv&GC_per_loc)".
+  - iExists ∅, ζ. rewrite map_union_empty. iFrame.
+    repeat iSplit; try iPureIntro.
+    + unfold lloc_map_pubs. rewrite omap_empty. done.
+    + by rewrite map_empty_union.
+    + apply map_disjoint_empty_l.
+    + done.
+    + intros γ; split.
+      * rewrite dom_empty_L. intros []%elem_of_empty.
+      * intros (ℓ&Vs&[]%lookup_empty_Some&_).
+    + intros ℓ Vs γ blk H1 []%lookup_empty_Some.
+  - rewrite lloc_map_pubs_insert_pub.
+    iPoseProof (big_sepM_insert with "GC_per_loc") as "((%vs&%tg&%lvs&[(Hℓ&%Hγζ)|[(%Hℓσ&Hγ&Hrest&->)|[(%Hnone1&%Hnone2)|(%Hnone1&%Hnone2)]]])&GC_per_loc)".
+    1: apply lloc_map_pubs_lookup_None; left; done.
+    + iDestruct (gen_heap_valid with "GCσMLv Hℓ") as %Hℓσ.
+      iDestruct (IH ζ with "[$GCζauth $Hplus $GC_per_loc $GCσMLv $GCχauth]") as "(%ζσ&%ζvirt&GCχauth&GCζauth&Hownres&HχNone&->&%Hdisj&GCσMLv&(#_&%Hstore1)&%Hstore2)".
+      1: etransitivity; first apply insert_subseteq; done.
+      iExists ζσ, ζvirt. iFrame "GCζauth GCσMLv GCχauth Hownres".
+      iSplitL; last repeat iSplit; try iPureIntro.
+      * iApply big_sepM_insert; first (apply lloc_map_pubs_lookup_None; left; done).
+        iFrame "HχNone". iExists vs, tg, lvs. iLeft. iFrame. iPureIntro.
+        apply lookup_union_Some_inv_r in Hγζ; first done.
+        destruct (ζσ !! γ) eqn:Heq; last done. exfalso.
+        eapply elem_of_dom_2 in Heq. apply Hstore1 in Heq as (ℓ'&Vs'&HH1&HH2); simplify_eq.
+      * done.
+      * done.
+      * done.
+      * intros γ'; specialize (Hstore1 γ') as [Hs1L Hs1R]; split.
+        -- intros Hdom. destruct (Hs1L Hdom) as (ℓ'&Vs'&HH1&HH2).
+           exists ℓ',Vs'. split; last done. rewrite lookup_insert_ne; first done.
+           intros ->; congruence.
+        -- intros (ℓ'&Vs'&[(HH1a&HH1b)|(HH1a&HH1b)]%lookup_insert_Some&HH2).
+           2: apply Hs1R; by repeat eexists.
+           simplify_eq.
+      * intros ℓ' vs' γ' blk' HH1 [(HH2a&HH2b)|(HH2a&HH2b)]%lookup_insert_Some HH3; first by simplify_eq.
+        by eapply Hstore2.
+    + iPoseProof (lstore_own_vblock_M_as_mut with "Hγ") as "(Hγ&%ℓ'&Hℓγ)".
+      iPoseProof (lstore_own_mut_of with "GCζauth Hγ") as "#(%Hζγ&_)".
+      iPoseProof (lstore_own_mut_to_elem with "Hγ") as "Hγ".
+      eapply lookup_union_Some_raw in Hζγ as [Hζγ|(Hne&Hζγ)].
+      1: { iPoseProof (big_sepM_lookup_acc with "Hplus") as "(Hcontr&_)"; first done.
+           rewrite /lstore_own_elem /mutability. cbn. iPoseProof (ghost_map_elem_ne with "Hcontr Hγ") as "%H". done. }
+      iPoseProof (GC_per_loc_delete_ζ with "GC_per_loc") as "GC_per_loc".
+      1: apply lloc_map_pubs_lookup_None; by left.
+      iPoseProof (block_sim_arr_auth_is_val_strong with "GCχauth GCζauth Hplus Hrest") as "%His_val".
+      1: by erewrite map_empty_union. 1: apply map_disjoint_empty_l.
+      iDestruct (IH (delete γ ζ) (<[ γ := _ ]> ζplus) with "[GCζauth Hplus Hγ $GC_per_loc $GCσMLv $GCχauth]") as "(%ζσ&%ζvirt&GCχauth&GCζauth&Hplus&HχNone&%Heqζ&%Hdisj&GCσMLv&(#_&%Hstore1)&%Hstore2)".
+      1: etransitivity; first apply insert_subseteq; done.
+      { rewrite union_insert_delete; try done. iFrame. iApply big_sepM_insert; try done. iFrame. }
+      rewrite union_insert_delete; try done.
+      rewrite -insert_union_l insert_union_r; last done.
+      iPoseProof (lloc_own_pub_of with "GCχauth Hℓγ") as "%Hℓ'γχ".
+      assert (χ !! γ = Some (LlocPublic ℓ)) as Hℓγχ by (by eapply lookup_weaken; last apply Hsub; eapply lookup_insert).
+      assert (ℓ' = ℓ) as -> by congruence.
+      iExists (<[ γ := (Bvblock (Mut, (TagDefault, lvs))) ]> ζσ), ζvirt.
+      iFrame "GCζauth GCσMLv GCχauth Hplus".
+      assert (ζvirt !! γ = None) as HζγvNone.
+      { destruct (ζvirt !! γ) eqn:Heq; last done. exfalso.
+        eapply elem_of_dom_2, elem_of_union_r, dom_union in Heq.
+        erewrite <-Heqζ, dom_delete_L in Heq. set_solver. }
+      iSplitL; last repeat iSplit; try iPureIntro.
+      * iApply big_sepM_insert; first (apply lloc_map_pubs_lookup_None; left; done).
+        iFrame "HχNone". iExists vs, TagDefault, lvs. iRight. iFrame. by iPureIntro.
+      * by rewrite <- insert_union_l, <-Heqζ, insert_delete.
+      * apply map_disjoint_insert_l_2; done.
+      * done.
+      * intros γ'; specialize (Hstore1 γ') as [Hs1L Hs1R]; split.
+        -- rewrite dom_insert_L. intros [->%elem_of_singleton|Hdom]%elem_of_union.
+           ++ exists ℓ, vs. by rewrite lookup_insert.
+           ++ destruct (Hs1L Hdom) as (ℓ'&Vs'&HH1&HH2).
+              exists ℓ',Vs'. split; last done. rewrite lookup_insert_ne; first done.
+              intros ->; congruence.
+        -- rewrite dom_insert_L.
+           intros (ℓ'&Vs'&[(HH1a&HH1b)|(HH1a&HH1b)]%lookup_insert_Some&HH2); eapply elem_of_union.
+           2: right; apply Hs1R; by repeat eexists.
+           left. eapply elem_of_singleton. done.
+      * intros ℓ' vs' γ' blk' HH1 [(HH2a&HH2b)|(HH2a&HH2b)]%lookup_insert_Some HH3.
+        -- simplify_eq. by econstructor.
+        -- eapply (is_heap_elt_weaken χ (delete γ ζ)); [|done|by apply delete_subset].
+           eapply Hstore2; try done. by rewrite lookup_delete_ne.
+    + iDestruct (IH ζ with "[$GCζauth $Hplus $GC_per_loc $GCσMLv $GCχauth]") as "(%ζσ&%ζvirt&GCχauth&GCζauth&Hownres&HχNone&->&%Hdisj&GCσMLv&(#_&%Hstore1)&%Hstore2)".
+      1: etransitivity; first apply insert_subseteq; done.
+      iPoseProof (lloc_own_auth_get_pub with "GCχauth") as "#Hsim".
+      1: (eapply lookup_weaken; last apply Hsub); by erewrite lookup_insert.
+      iExists ζσ, ζvirt. iFrame "GCζauth GCσMLv GCχauth Hownres".
+      iSplitL; last repeat iSplit; try iPureIntro.
+      * iApply big_sepM_insert; first (apply lloc_map_pubs_lookup_None; left; done).
+        iFrame "HχNone". iExists vs, tg, lvs. iRight. iFrame "Hsim". iPureIntro.
+        eapply lookup_union_None in Hnone2 as [HH1 HH2]; done.
+      * done.
+      * done.
+      * done.
+      * intros γ'; specialize (Hstore1 γ') as [Hs1L Hs1R]; split.
+        -- intros Hdom. destruct (Hs1L Hdom) as (ℓ'&Vs'&HH1&HH2).
+           exists ℓ',Vs'. split; last done. rewrite lookup_insert_ne; first done.
+           intros ->; congruence.
+        -- intros (ℓ'&Vs'&[(HH1a&HH1b)|(HH1a&HH1b)]%lookup_insert_Some&HH2).
+           2: apply Hs1R; by repeat eexists.
+           simplify_eq.
+      * intros ℓ' vs' γ' blk' HH1 [(HH2a&HH2b)|(HH2a&HH2b)]%lookup_insert_Some HH3; first by simplify_eq.
+        by eapply Hstore2.
+    + iDestruct (IH ζ with "[$GCζauth $Hplus $GC_per_loc $GCσMLv $GCχauth]") as "(%ζσ&%ζvirt&GCχauth&GCζauth&Hownres&HχNone&->&%Hdisj&GCσMLv&(#_&%Hstore1)&%Hstore2)".
+      1: etransitivity; first apply insert_subseteq; done.
+      iPoseProof (lloc_own_auth_get_pub with "GCχauth") as "#Hsim".
+      1: (eapply lookup_weaken; last apply Hsub); by erewrite lookup_insert.
+      iExists ζσ, ζvirt. iFrame "GCζauth GCσMLv GCχauth Hownres".
+      iSplitL; last repeat iSplit; try iPureIntro.
+      * iApply big_sepM_insert; first (apply lloc_map_pubs_lookup_None; left; done).
+        iFrame "HχNone". iExists vs, tg, lvs. iRight. iFrame "Hsim". iPureIntro.
+        eapply lookup_union_None in Hnone2 as [HH1 HH2]; done.
+      * done.
+      * done.
+      * done.
+      * intros γ'; specialize (Hstore1 γ') as [Hs1L Hs1R]; split.
+        -- intros Hdom. destruct (Hs1L Hdom) as (ℓ'&Vs'&HH1&HH2).
+           exists ℓ',Vs'. split; last done. rewrite lookup_insert_ne; first done.
+           intros ->; congruence.
+        -- intros (ℓ'&Vs'&[(HH1a&HH1b)|(HH1a&HH1b)]%lookup_insert_Some&HH2).
+           2: apply Hs1R; by repeat eexists.
+           simplify_eq.
+      * intros ℓ' vs' γ' blk' HH1 [(HH2a&HH2b)|(HH2a&HH2b)]%lookup_insert_Some HH3; first by simplify_eq.
+        by eapply Hstore2.
+  - rewrite lloc_map_pubs_insert_foreign -lloc_map_pubs_delete delete_notin. 2: done.
+    iDestruct (IH with "[$GCζauth $GC_per_loc $Hplus $GCσMLv $GCχauth]") as "(%ζσ&%ζvirt&GCχauth&GCζauth&Hplus&HχNone&%Heqζ&%Hdisj&GCσMLv&(#_&%Hstore1)&%Hstore2)".
+    1: etransitivity; first apply insert_subseteq; done.
+    iExists ζσ, ζvirt. iFrame.
+    iPureIntro; split_and!.
+    + done.
+    + done.
+    + done.
+    + intros γ'; destruct (Hstore1 γ') as [HL HR]; split.
+      * intros H; destruct (HL H) as (ℓ&Vs&H1&H2). exists ℓ,Vs. split; last done.
+        rewrite lookup_insert_ne; first done. intros ->; simplify_eq; done.
+      * intros (ℓ&Vs&[(->&H1)|(H1a&H1b)]%lookup_insert_Some&H2).
+        1: congruence.
+        apply HR; by repeat eexists.
+    + intros ℓ vs γ' blk H1 [(->&H2)|(H2a&H2b)]%lookup_insert_Some H3.
+      1: congruence.
+      eapply Hstore2; done.
+  - rewrite lloc_map_pubs_insert_priv -lloc_map_pubs_delete delete_notin. 2: done.
+    iDestruct (IH with "[$GCζauth $GC_per_loc $Hplus $GCσMLv $GCχauth]") as "(%ζσ&%ζvirt&GCχauth&GCζauth&Hplus&HχNone&%Heqζ&%Hdisj&GCσMLv&(#_&%Hstore1)&%Hstore2)".
+    1: etransitivity; first apply insert_subseteq; done.
+    iExists ζσ, ζvirt. iFrame.
+    iPureIntro; split_and!.
+    + done.
+    + done.
+    + done.
+    + intros γ'; destruct (Hstore1 γ') as [HL HR]; split.
+      * intros H; destruct (HL H) as (ℓ&Vs&H1&H2). exists ℓ,Vs. split; last done.
+        rewrite lookup_insert_ne; first done. intros ->; simplify_eq; done.
+      * intros (ℓ&Vs&[(->&H1)|(H1a&H1b)]%lookup_insert_Some&H2).
+        1: congruence.
+        apply HR; by repeat eexists.
+    + intros ℓ vs γ' blk H1 [(->&H2)|(H2a&H2b)]%lookup_insert_Some H3.
+      1: congruence.
+      eapply Hstore2; done.
+Qed.
+
+Lemma scrub_zeta ζσ ζvirt :
+    ⌜ζσ ##ₘ ζvirt⌝
+  ∗ lstore_own_auth (ζσ ∪ ζvirt)
+  ∗ ([∗ map] γ↦b ∈ ζσ, ghost_map_elem wrapperG_γζvirt γ (DfracOwn 1) b)
+  ⊢ |==> lstore_own_auth ζvirt.
+Proof.
+  induction ζσ as [|γ blk ζσ Hnone IH] using map_ind;
+  iIntros "(%Hdisj&Hζ&Hdel)".
+  - by rewrite map_empty_union.
+  - rewrite -insert_union_l. iPoseProof (big_sepM_insert with "Hdel") as "(HH&Hdel)"; first done.
+    rewrite /lstore_own_auth. iNamed "Hζ".
+    iMod (ghost_map_delete with "Hζgmap HH") as "Hζgmap".
+    assert (ζvirt !! γ = None) as Hnonev.
+    { destruct (ζvirt !! γ) eqn:Heq; last done.
+      eapply map_disjoint_Some_r in Heq; last done. by rewrite lookup_insert in Heq. }
+    iAssert (lstore_own_auth (ζσ ∪ ζvirt)) with "[Hζgmap]" as "Hζ".
+    { rewrite /lstore_own_auth /named. rewrite delete_insert; first iFrame.
+      1: rewrite /lstore_immut_blocks map_filter_insert; destruct decide as [Heq|Hne].
+      1: iPoseProof (big_sepM_insert with "Hζimmut") as "(_&$)"; apply map_filter_lookup_None_2; left.
+      2: rewrite delete_notin; first done.
+      all: apply lookup_union_None_2; done. }
+    iApply (IH). iFrame. iPureIntro.
+    eapply map_disjoint_insert_l; done.
+Qed.
+
 Lemma wrap_interp_c_to_ml ws ρc mem θ vs lvs :
   Forall2 (repr_lval θ) lvs ws →
   wrap_state_interp (Wrap.CState ρc mem) -∗
@@ -32,11 +238,12 @@ Lemma wrap_interp_c_to_ml ws ρc mem θ vs lvs :
   ⌜c_to_ml ws ρc mem vs ρml σ⌝ ∗
   |==> wrap_state_interp (Wrap.MLState ρml σ) ∗ not_at_boundary.
 Proof using.
-  iIntros (Hlv) "Hσ HGC Hnb #Hblk".
+  iIntros (Hlv) "Hσ HGC Hnb #Hblk". 
   iNamed "Hσ". iNamed "SIC". iNamed "HGC". simplify_eq. SI_GC_agree.
+  iNamed "HSI_GC". iNamed "HSI_block_level".
 
-  iAssert (⌜Forall2 (is_val χvirt (ζσ ∪ ζvirt)) vs lvs⌝)%I as "%Hval".
-  1: by iApply (block_sim_arr_auth_is_val with "GCχvirt GCζvirt Hblk").
+  iAssert (⌜Forall2 (is_val χ_future ζ_future) vs lvs⌝)%I as "%Hval".
+  1: iApply (block_sim_arr_auth_is_val_simple with "GCχauth GCζauth Hblk").
   iAssert (⌜∀ k lv, roots_m !! k = Some lv →
             ∃ w, mem !! k = Some (Storing w) ∧ repr_lval (θC ρc) lv w⌝)%I as "%Hroots".
   1: { iIntros (kk vv Hroots).
@@ -45,10 +252,13 @@ Proof using.
   apply map_Forall_lookup_2 in Hroots.
   destruct (make_repr (θC ρc) roots_m mem) as [privmem Hpriv]; try done.
 
+  iPoseProof (GC_SI_to_C σMLvirt ζ_future ∅ χ_future with "[$GCχauth $GCσMLv $GC_per_loc GCζauth]") as "(%ζσ&%ζvirt&GCχauth&GCζauth&Hownres&HχNone&->&%Hdisj&GCσMLv&(#_&%Hstore1)&%Hstore2)".
+  { rewrite map_empty_union. iFrame. by repeat iSplit. }
+
   iExists (WrapstateML _ _ _ _), _. iSplit.
   { iPureIntro. unfold c_to_ml. cbn.
     eexists σMLvirt, _, _, (ζσ ∪ ζvirt), ζσ. split_and!; eauto.
-    by rewrite map_union_comm. }
+    1: by rewrite map_union_comm. by split. }
 
   iMod (ghost_var_update_halves with "Hnb SIbound") as "(Hb & SIbound)".
   iMod (ghost_var_update_halves with "GCζ SIζ") as "(GCζ & SIζ)".
@@ -57,13 +267,381 @@ Proof using.
   iMod (ghost_var_update_halves with "GCroots SIroots") as "(GCroots & SIroots)".
   iMod (set_to_none with "HσC GCrootspto") as "(HσC & GCrootspto)"; first done.
 
+  rewrite !map_empty_union.
+  iMod (scrub_zeta with "[$Hownres $GCζauth]") as "GCζauth"; first done.
+
   iModIntro. iSplitR "SIbound"; last by iFrame "SIbound".
   rewrite /= /named. iFrame "GCσMLv".
-  unfold private_state_interp, ML_state_interp, GC_token_remnant, named; cbn.
-  iFrame. iPureIntro; split_and!.
-  1: destruct Hχvirt as (_ & HHH); apply HHH.
-  1: apply Hother_blocks.
-  1: destruct Hpriv as (mem_r & ->%repr_roots_dom & Hpriv2 & Hpriv3); by apply map_disjoint_dom.
+  unfold private_state_interp, ML_state_interp, GC_remnant_ML, SI_block_level_ML, SI_GC_ML, named; cbn.
+  iFrame. iSplitL.
+  { iExists _, _. iFrame. repeat iSplit.
+    - iPureIntro. rewrite dom_union_L in Hother_blocks. set_solver.
+    - by iApply big_sepM_dom.
+    - iPureIntro. apply Hχfuture. }
+  iPureIntro.
+  destruct Hpriv as (mem_r & ->%repr_roots_dom & Hpriv2 & Hpriv3); by apply map_disjoint_dom.
+Qed.
+
+Lemma is_store_blocks_delete_from_sigma γ ll (ζσ ζrest : lstore) χind χnew χplus (σ : store) :
+   ζσ ##ₘ ζrest
+ → γ ∈ dom ζσ
+ → χind !! γ = None
+ → <[γ:=ll]> χind ⊆ χnew
+ → (∀ γ', γ' ∈ dom ζσ ↔ (∃ ℓ Vs, <[γ:=ll]> χind !! γ' = Some (LlocPublic ℓ) ∧ σ !! ℓ = Some (Some Vs)))
+ → χnew ⊆ χplus
+ → (∀ ℓ vs γ' blk, σ !! ℓ = Some (Some vs) → χnew !! γ' = Some (LlocPublic ℓ) → (ζσ ∪ ζrest) !! γ' = Some blk → is_heap_elt χplus (ζσ ∪ ζrest) vs blk)
+ → (∀ ℓ vs γ' blk, σ !! ℓ = Some (Some vs) → χnew !! γ' = Some (LlocPublic ℓ) → (delete γ ζσ ∪ ζrest) !! γ' = Some blk → is_heap_elt χplus (delete γ ζσ ∪ ζrest) vs blk).
+Proof.
+  intros H1 Hdom Hndom Hsub H2 Hnew H3 ℓ Vs γ' blk HH1 HH2 HH3.
+  unshelve epose proof (H3 ℓ Vs γ' blk HH1 HH2 _) as Helt.
+  { eapply lookup_union_Some in HH3 as [HH3|HH3].
+    - apply lookup_union_Some_l. apply lookup_delete_Some in HH3 as (Hne&HH3); done.
+    - by apply lookup_union_Some_r.
+    - by apply map_disjoint_delete_l. }
+  assert (delete γ ζσ ∪ ζrest = delete γ (ζσ ∪ ζrest)) as Hdel.
+  { rewrite delete_union. f_equal. rewrite delete_notin; try done.
+    eapply elem_of_dom in Hdom as [blkγ Hdom].
+    eapply map_disjoint_Some_l; done. }
+  inversion Helt; simplify_eq. econstructor.
+  eapply Forall2_impl; first eassumption.
+  assert (∃ ζ, ζ = ζσ ∪ ζrest) as [ζ Heqζ] by by eexists.
+  rewrite -Heqζ.
+  intros V v; induction 1; try by econstructor. all: econstructor; subst ζ.
+  1,4,6,8: rewrite Hdel; rewrite lookup_delete_ne; first eassumption.
+  1-4: intros <-; destruct (H2 γ) as [H2'' _]; destruct H2'' as (ℓ''&Vs''&HHH1&HHH2); first done;
+       rewrite lookup_insert in HHH1; simplify_eq;
+       unshelve epose proof (H3 ℓ'' Vs'' γ _ HHH2 _ _) as Helt2; [|eapply lookup_weaken; last eassumption; by rewrite lookup_insert|done|]; inversion Helt2; simplify_eq.
+  1: by eapply IHis_val1.
+  1: by eapply IHis_val2.
+  1: by eapply IHis_val.
+  1: by eapply IHis_val.
+Qed.
+
+Lemma gmap_new_elems {A B : Type} `{Countable A} (m1 m2 : gmap A B) : m1 ⊆ m2 → ∃ mr, m2 = m1 ∪ mr ∧ m1 ##ₘ mr.
+Proof.
+  exists (filter (fun '(k,_) => (m1 !! k) = None) m2). split.
+  - eapply map_eq_iff. intros k. rewrite lookup_union. destruct (m1 !! k) eqn:Heq.
+    + cbn. rewrite map_filter_lookup_None_2.
+      * cbn. by eapply lookup_weaken.
+      * right. intros  _ _ Heq2. simplify_eq.
+    + rewrite union_with_left_id. rewrite map_filter_lookup. destruct (m2 !! k); cbn; last done.
+      by rewrite option_guard_True.
+  - apply map_disjoint_spec. intros k v1 v2 HH1 (_&HH2)%map_filter_lookup_Some. simplify_eq.
+Qed.
+
+(* Step 1: convert the per_location_invariant for all already known mappings in χ *)
+(* Notice that this has no χold and χnew *)
+Lemma GC_SI_to_ML_one σMLvirt ζvirt ζσ ζnewimm χ χplus:
+    ⌜ζvirt ##ₘ ζnewimm⌝ ∗ ⌜ζσ ##ₘ ζnewimm⌝ ∗ ⌜ζvirt ##ₘ ζσ⌝
+  ∗ ⌜(∀ γ, γ ∈ dom ζσ ↔ (∃ ℓ Vs, χ !! γ = Some (LlocPublic ℓ) ∧ σMLvirt !! ℓ = Some (Some Vs)))⌝ ∗ ⌜lloc_map_inj χ⌝ ∗ ⌜χ ⊆ χplus⌝
+  ∗ ⌜∀ ℓ vs γ blk, σMLvirt !! ℓ = Some (Some vs) → χ !! γ = Some (LlocPublic ℓ) → (ζσ ∪ (ζvirt ∪ ζnewimm)) !! γ = Some blk → is_heap_elt χplus (ζσ ∪ (ζvirt ∪ ζnewimm)) vs blk⌝
+  ∗ ⌜dom ζvirt ⊆ dom χ⌝
+  ∗ lloc_own_auth χplus
+  ∗ state_interp (σMLvirt : language.language.state ML_lang)
+  ∗ lstore_own_auth (ζvirt ∪ ζnewimm)
+  ∗ ([∗ map] γ↦ℓ ∈ lloc_map_pubs χ, per_location_invariant_ML ζvirt γ ℓ)
+ ⊢ |==> lstore_own_auth (ζσ ∪ (ζvirt ∪ ζnewimm))
+  ∗ ([∗ map] γ↦ℓ ∈ lloc_map_pubs χ, per_location_invariant (ζσ ∪ ζvirt) σMLvirt γ ℓ)
+  ∗ lloc_own_auth χplus
+  ∗ state_interp (σMLvirt : language.language.state ML_lang).
+Proof.
+  iIntros "(%Hdisj1&%Hdisj2&%Hdisj3&%Hbl2&%Hinj&%Hplus&%Hisstore&%Hother_blocks&GCχauth&GCζauth&GCσMLv&GC_per_loc)".
+  assert (∃ χind, χind ⊆ χ ∧ χ = χind) as (χind&Hsub&Heqind).
+  1: eexists _; split; last done; done.
+  iStopProof.
+  rewrite /named. revert ζσ Hdisj2 Hdisj3 Hbl2 Hisstore Hother_blocks Hinj Hplus Hsub.
+  rewrite {1 7 8} Heqind. clear Heqind.
+  induction χind as [|γ [ℓ|fid|] χind Hnone IH] using map_ind;
+  intros ζσ Hdisj2 Hdisj3 Hbl2 Hisstore Hother_blocks Hinj Hplus Hsub;
+  iIntros "(GCχauth&GCσMLv&GCζauth&GC_per_loc)".
+  - rewrite lloc_map_pubs_empty.
+    assert (ζσ = ∅) as ->.
+    1: { apply map_empty. intros γ. eapply not_elem_of_dom. intros Hdom.
+         apply Hbl2 in Hdom as (?&?&[]%lookup_empty_Some&_). }
+    rewrite map_empty_union. iFrame. iModIntro. done.
+  - rewrite lloc_map_pubs_insert_pub.
+    iPoseProof (big_sepM_insert with "GC_per_loc") as "((%vs&%tg&%lvs&[(Hnℓ&%Hγ)|(%Hne&Hsim)])&GC_per_loc)".
+    + apply lloc_map_pubs_lookup_None. by left.
+    + assert (ζσ !! γ = None) by by eapply map_disjoint_Some_l.
+      iMod (IH with "[$GCχauth $GCσMLv $GCζauth $GC_per_loc]") as "(GCχauth&GCσMLv&GCζauth&GC_per_loc)"; try done.
+      * intros γ'; destruct (Hbl2 γ') as [HblL HblR]; split.
+        -- intros Hg; destruct (HblL Hg) as (ℓ'&Vs&HH1&HH2). repeat eexists; try done.
+           rewrite lookup_insert_ne in HH1; try done. intros ->; by eapply not_elem_of_dom in H.
+        -- intros (ℓ'&Vs&HH1&HH2). eapply HblR. repeat eexists; try done.
+           rewrite lookup_insert_ne; try done. intros ->; simplify_eq.
+      * apply map_subseteq_spec. intros γ' v1 Hv1. eapply lookup_weaken. 2: exact Hsub.
+        rewrite lookup_insert_ne; try done. intros ->; simplify_eq.
+      * iModIntro. iFrame. iApply big_sepM_insert; first (apply lloc_map_pubs_lookup_None; by left). iFrame.
+        iExists vs, tg, lvs. iLeft. iFrame. iPureIntro. by rewrite lookup_union_r.
+    + destruct (σMLvirt !! ℓ) as [[Vs|]|] eqn:Heq.
+      * assert (γ ∈ dom ζσ) as [blk Hblk]%elem_of_dom.
+        1: eapply Hbl2; repeat eexists; try done; by rewrite lookup_insert.
+        unshelve epose proof (Hisstore ℓ Vs γ blk Heq _ _) as Helt.
+        1: eapply lookup_weaken; last exact Hsub; by rewrite lookup_insert.
+        1: by erewrite lookup_union_Some_l.
+        iMod (IH (delete γ ζσ) with "[$GCχauth $GCσMLv $GCζauth $GC_per_loc]") as "(GCζauth&GC_per_loc&GCχauth&GCσMLv)"; try done.
+        1: by apply map_disjoint_delete_l.
+        1: by apply map_disjoint_delete_r.
+        { intros γ'; destruct (Hbl2 γ') as [HHL HHR]; split; rewrite dom_delete_L.
+         - intros (H&Hnee%not_elem_of_singleton)%elem_of_difference.
+           destruct (HHL H) as (ℓ'&Vs'&HH1&HH2). repeat eexists; try done. by rewrite lookup_insert_ne in HH1.
+         - intros (ℓ'&Vs'&HH1&HH2). apply elem_of_difference.
+           assert (γ ≠ γ') as Hnee.
+           1: intros ->; simplify_eq. split.
+           1: eapply HHR; repeat eexists; last done; by rewrite lookup_insert_ne.
+           by eapply not_elem_of_singleton. }
+        1: { eapply is_store_blocks_delete_from_sigma. 4: eassumption. all: try done. 2: by eapply elem_of_dom_2. by apply map_disjoint_union_r_2. }
+        1: apply map_subseteq_spec; intros γ' v1 Hv1; eapply lookup_weaken; last exact Hsub;
+           rewrite lookup_insert_ne; try done; intros ->; simplify_eq.
+        assert (ζnewimm !! γ = None) by by eapply map_disjoint_Some_l.
+        assert ((delete γ ζσ ∪ (ζvirt ∪ ζnewimm)) = delete γ (ζσ ∪ (ζvirt ∪ ζnewimm))) as Hdel.
+        { rewrite ! delete_union. f_equal. rewrite !delete_notin; done. }
+        iMod (lstore_own_insert _ _ blk with "GCζauth") as "(GCζauth&GCnew)".
+        1: erewrite Hdel, lookup_delete; done.
+        inversion Helt; simplify_eq.
+        rewrite !Hdel insert_delete.
+        2: by apply lookup_union_Some_l.
+        iPoseProof (block_sim_arr_of_auth_strong _ _ Vs lvs0 with "GCχauth GCζauth") as "#Hsimvs".
+        { eapply Forall2_impl; first eassumption. intros x y HH. eapply is_val_mono; last done; done. }
+        iPoseProof (lloc_own_auth_get_pub with "GCχauth") as "#Hsimell".
+        1: eapply lookup_weaken; last (etransitivity; try exact Hsub; done); by erewrite lookup_insert.
+        iModIntro. iFrame. iApply big_sepM_insert.
+        1: apply lloc_map_pubs_lookup_None; by left.
+        iSplitR "GC_per_loc".
+        -- iExists _, _, _. iRight. iLeft. iFrame. iSplitL; first done. iSplitL; first by iExists _.
+           iSplit; done.
+        -- iPoseProof (GC_per_loc_modify_ζ with "GC_per_loc") as "GC_per_loc".
+           1: apply lloc_map_pubs_lookup_None; by left.
+           erewrite insert_union_l. by rewrite insert_delete.
+      * assert (γ ∉ dom ζσ) as Hnin%not_elem_of_dom.
+        1: intros H; apply Hbl2 in H as (ℓ'&Vs&HH1&HH2); rewrite lookup_insert in HH1; simplify_eq.
+        iMod (IH with "[$GCχauth $GCσMLv $GCζauth $GC_per_loc]") as "(GCχauth&GCσMLv&GCζauth&GC_per_loc)"; try done.
+        -- intros γ'; destruct (Hbl2 γ') as [HblL HblR]; split.
+           ++ intros Hg; destruct (HblL Hg) as (ℓ'&Vs&HH1&HH2). repeat eexists; try done.
+              rewrite lookup_insert_ne in HH1; try done. intros ->; eapply not_elem_of_dom in Hnin; done.
+           ++ intros (ℓ'&Vs&HH1&HH2). eapply HblR. repeat eexists; try done.
+              rewrite lookup_insert_ne; try done. intros ->; simplify_eq.
+        -- apply map_subseteq_spec. intros γ' v1 Hv1. eapply lookup_weaken. 2: exact Hsub.
+           rewrite lookup_insert_ne; try done. intros ->; simplify_eq.
+        -- iModIntro. iFrame. iApply big_sepM_insert; first (apply lloc_map_pubs_lookup_None; by left). iFrame.
+           iExists vs, tg, lvs. iRight. iRight. iRight. iPureIntro; split; first done.
+           by apply lookup_union_None_2.
+      * assert (γ ∉ dom ζσ) as Hnin%not_elem_of_dom.
+        1: intros H; apply Hbl2 in H as (ℓ'&Vs&HH1&HH2); rewrite lookup_insert in HH1; simplify_eq.
+        iMod (IH with "[$GCχauth $GCσMLv $GCζauth $GC_per_loc]") as "(GCχauth&GCσMLv&GCζauth&GC_per_loc)"; try done.
+        -- intros γ'; destruct (Hbl2 γ') as [HblL HblR]; split.
+           ++ intros Hg; destruct (HblL Hg) as (ℓ'&Vs&HH1&HH2). repeat eexists; try done.
+              rewrite lookup_insert_ne in HH1; try done. intros ->; eapply not_elem_of_dom in Hnin; done.
+           ++ intros (ℓ'&Vs&HH1&HH2). eapply HblR. repeat eexists; try done.
+              rewrite lookup_insert_ne; try done. intros ->; simplify_eq.
+        -- apply map_subseteq_spec. intros γ' v1 Hv1. eapply lookup_weaken. 2: exact Hsub.
+           rewrite lookup_insert_ne; try done. intros ->; simplify_eq.
+        -- iModIntro. iFrame. iApply big_sepM_insert; first (apply lloc_map_pubs_lookup_None; by left). iFrame.
+           iExists vs, tg, lvs. iRight. iRight. iLeft. iPureIntro; split; first done.
+           by apply lookup_union_None_2.
+  - rewrite lloc_map_pubs_insert_foreign -lloc_map_pubs_delete delete_notin; last done.
+    iApply (IH); try done.
+    + intros γ'; destruct (Hbl2 γ') as [HblL HblR]; split.
+      * intros Hg; destruct (HblL Hg) as (ℓ'&Vs&[(_&HH1)|(HH1L&HH1R)]%lookup_insert_Some&HH2); first simplify_eq.
+        by repeat eexists.
+      * intros (ℓ'&Vs&HH1&HH2). eapply HblR. repeat eexists; try done.
+        rewrite lookup_insert_ne; try done. intros ->; simplify_eq.
+    + apply map_subseteq_spec. intros γ' v1 Hv1. eapply lookup_weaken. 2: exact Hsub.
+      rewrite lookup_insert_ne; try done. intros ->; simplify_eq.
+    + iFrame.
+  - rewrite lloc_map_pubs_insert_priv -lloc_map_pubs_delete delete_notin; last done.
+    iApply (IH); try done.
+    + intros γ'; destruct (Hbl2 γ') as [HblL HblR]; split.
+      * intros Hg; destruct (HblL Hg) as (ℓ'&Vs&[(_&HH1)|(HH1L&HH1R)]%lookup_insert_Some&HH2); first simplify_eq.
+        by repeat eexists.
+      * intros (ℓ'&Vs&HH1&HH2). eapply HblR. repeat eexists; try done.
+        rewrite lookup_insert_ne; try done. intros ->; simplify_eq.
+    + apply map_subseteq_spec. intros γ' v1 Hv1. eapply lookup_weaken. 2: exact Hsub.
+      rewrite lookup_insert_ne; try done. intros ->; simplify_eq.
+    + iFrame.
+Qed.
+
+(* Step 2: We got χold and χnew, we now add all mappings new in χnew *)
+Lemma GC_SI_to_ML_2 σMLvirt ζvirt ζσ ζnewimm χold χnew :
+    ⌜ζvirt ##ₘ ζnewimm⌝ ∗ ⌜ζσ ##ₘ ζnewimm⌝ ∗ ⌜ζvirt ##ₘ ζσ⌝
+  ∗ ⌜is_store_blocks χnew σMLvirt ζσ⌝
+  ∗ ⌜lloc_map_mono χold χnew⌝
+  ∗ ⌜is_private_blocks χnew ζnewimm⌝ ∗ ⌜is_store χnew (ζσ ∪ (ζvirt ∪ ζnewimm)) σMLvirt⌝ ∗ ⌜dom ζvirt ⊆ dom χold⌝
+  ∗ lloc_own_auth χnew
+  ∗ state_interp (σMLvirt : language.language.state ML_lang)
+  ∗ lstore_own_auth (ζvirt ∪ ζnewimm)
+  ∗ ([∗ map] γ↦ℓ ∈ lloc_map_pubs χold, per_location_invariant_ML ζvirt γ ℓ)
+ ⊢ |==> lstore_own_auth (ζσ ∪ (ζvirt ∪ ζnewimm))
+  ∗ ([∗ map] γ↦ℓ ∈ lloc_map_pubs χnew, per_location_invariant (ζσ ∪ ζvirt) σMLvirt γ ℓ)
+  ∗ lloc_own_auth χnew
+  ∗ state_interp (σMLvirt : language.language.state ML_lang).
+Proof.
+  iIntros "(%Hdisj1&%Hdisj2&%Hdisj3&%Hbl&%Hmono&%Hpriv&%Hisstore&%Hother_blocks&GCχauth&GCζauth&GCσMLv&GC_per_loc)".
+  destruct Hmono as [Hmono Hinj].
+  destruct Hbl as [Hbl1 Hbl2].
+  destruct (gmap_new_elems _ _ Hmono) as (χfresh&Heqfresh&Hχdisj).
+  assert (∃ χind, χind ⊆ χfresh ∧ χfresh = χind) as (χind&Hsub&Heqind).
+  1: eexists _; split; last done; done.
+  iStopProof.
+  rewrite /named. revert ζσ Hdisj2 Hdisj3 Hbl1 Hbl2 Hpriv Hisstore Hother_blocks Hmono Hinj Hsub Hχdisj.
+  subst χnew.
+  rewrite {2 10} Heqind. clear Heqind.
+  induction χind as [|γ [ℓ|fid|] χind Hnone IH] using map_ind;
+  intros ζσ Hdisj2 Hdisj3 Hbl1 Hbl2 Hpriv Hisstore Hother_blocks Hmono Hinj Hsub Hχdisj;
+  iIntros "(GCχauth&GCσMLv&GCζauth&GC_per_loc)".
+  2-4: assert (χold !! γ = None) as Hnold by (eapply map_disjoint_Some_r; first eassumption; eapply lookup_weaken; last eassumption; by erewrite lookup_insert).
+  - rewrite map_union_empty in Hbl2|-*.
+    iApply (GC_SI_to_ML_one).
+    iFrame. iPureIntro. split_and!; try done.
+    + intros γ1 γ2 ℓ H1 H2. apply Hinj.
+      all: eapply lookup_weaken; done.
+    + intros ℓ vs γ blk HH1 HH2 HH3. eapply Hisstore; try done.
+      by apply lookup_union_Some_l.
+  - rewrite -insert_union_r in Hbl2|-*; last done.
+    destruct (σMLvirt !! ℓ) as [[Vs|]|] eqn:Heqell.
+    + assert (γ ∈ dom ζσ) as [blk Hblk]%elem_of_dom.
+      1: eapply Hbl2; repeat eexists; try done; by rewrite lookup_insert.
+      unshelve epose proof (Hisstore ℓ Vs γ blk Heqell _ _) as Helt.
+      1: eapply lookup_union_Some_r; first done; eapply lookup_weaken; last exact Hsub; by rewrite lookup_insert.
+      1: by erewrite lookup_union_Some_l.
+      iMod (IH (delete γ ζσ) with "[$GCχauth $GCσMLv $GCζauth $GC_per_loc]") as "(GCζauth&GC_per_loc&GCχauth&GCσMLv)"; try done.
+      1: by apply map_disjoint_delete_l.
+      1: by apply map_disjoint_delete_r.
+      { intros γ'; destruct (Hbl2 γ') as [HHL HHR]; split; rewrite dom_delete_L.
+       - intros (H&Hnee%not_elem_of_singleton)%elem_of_difference.
+         destruct (HHL H) as (ℓ'&Vs'&HH1&HH2). repeat eexists; try done. by rewrite lookup_insert_ne in HH1.
+       - intros (ℓ'&Vs'&HH1&HH2); apply elem_of_difference.
+         assert (γ ≠ γ') as Hnee.
+         1: eapply lookup_union_Some_raw in HH1 as [HH1|(HHr&HH1)]; intros ->; simplify_eq.
+         split; last by eapply not_elem_of_singleton.
+         eapply HHR; repeat eexists; last done; by rewrite lookup_insert_ne. }
+      1: { refine (is_store_blocks_delete_from_sigma _ _ _ _ (χold ∪ χind) _ _ _ _ _ _ _ _ _  Hisstore).
+           - by apply map_disjoint_union_r_2.
+           - by eapply elem_of_dom_2.
+           - by eapply lookup_union_None_2.
+           - erewrite insert_union_r; last done. eapply map_union_mono_l. done.
+           - eapply Hbl2.
+           - done. }
+      1: apply map_subseteq_spec; intros γ' v1 Hv1; eapply lookup_weaken; last exact Hsub;
+         rewrite lookup_insert_ne; try done; intros ->; simplify_eq.
+      assert (ζnewimm !! γ = None) by by eapply map_disjoint_Some_l.
+      assert (ζvirt !! γ = None) by by eapply map_disjoint_Some_l.
+      assert ((delete γ ζσ ∪ (ζvirt ∪ ζnewimm)) = delete γ (ζσ ∪ (ζvirt ∪ ζnewimm))) as Hdel.
+      { rewrite ! delete_union. f_equal. rewrite !delete_notin; done. }
+      iMod (lstore_own_insert _ _ blk with "GCζauth") as "(GCζauth&GCnew)".
+      1: erewrite Hdel, lookup_delete; done.
+      inversion Helt; simplify_eq.
+      rewrite !Hdel insert_delete.
+      2: by apply lookup_union_Some_l.
+      iPoseProof (block_sim_arr_of_auth_strong _ _ Vs lvs with "GCχauth GCζauth") as "#Hsimvs".
+      { eapply Forall2_impl; first eassumption. intros x y HH. eapply is_val_mono; last done; done. }
+      iPoseProof (lloc_own_auth_get_pub with "GCχauth") as "#Hsimell".
+      1: eapply lookup_union_Some_r; first done; eapply lookup_weaken; last exact Hsub; by erewrite lookup_insert.
+      iModIntro. iFrame. rewrite lloc_map_pubs_insert_pub. iApply big_sepM_insert.
+      1: apply lloc_map_pubs_lookup_None; left; eapply lookup_union_None_2; done.
+      iSplitR "GC_per_loc".
+      * iExists _, _, _. iRight. iLeft. iFrame. iFrame "Hsimvs". iSplit; first done.
+        iSplit; last done. by iExists _.
+      * iPoseProof (GC_per_loc_modify_ζ with "GC_per_loc") as "GC_per_loc".
+        1: apply lloc_map_pubs_lookup_None; left; eapply lookup_union_None_2; done.
+        erewrite insert_union_l. by rewrite insert_delete.
+    + assert (γ ∉ dom ζσ) as Hnin%not_elem_of_dom.
+      1: intros H; apply Hbl2 in H as (ℓ'&Vs&HH1&HH2); rewrite lookup_insert in HH1; simplify_eq.
+      iMod (IH with "[$GCχauth $GCσMLv $GCζauth $GC_per_loc]") as "(GCχauth&GCσMLv&GCζauth&GC_per_loc)"; try done.
+      * intros γ'; destruct (Hbl2 γ') as [HblL HblR]; split.
+        -- intros Hg; destruct (HblL Hg) as (ℓ'&Vs&HH1&HH2). repeat eexists; try done.
+           rewrite lookup_insert_ne in HH1; try done. intros ->; eapply not_elem_of_dom in Hnin; done.
+        -- intros (ℓ'&Vs'&HH1&HH2).
+           assert (γ ≠ γ') as Hnee.
+           1: eapply lookup_union_Some_raw in HH1 as [HH1|(HHr&HH1)]; intros ->; simplify_eq.
+           eapply HblR; repeat eexists; try done. by rewrite lookup_insert_ne.
+      * apply map_subseteq_spec. intros γ' v1 Hv1. eapply lookup_weaken. 2: exact Hsub.
+        rewrite lookup_insert_ne; try done. intros ->; simplify_eq.
+      * iModIntro. iFrame. rewrite lloc_map_pubs_insert_pub. iApply big_sepM_insert.
+        1: apply lloc_map_pubs_lookup_None; left; eapply lookup_union_None_2; done. iFrame.
+        iExists nil, TagDefault, nil. iRight. iRight. iRight. iPureIntro; split; first done.
+        apply lookup_union_None_2; try done. eapply not_elem_of_dom. intros H%Hother_blocks.
+        by eapply not_elem_of_dom in Hnold.
+    + assert (γ ∉ dom ζσ) as Hnin%not_elem_of_dom.
+      1: intros H; apply Hbl2 in H as (ℓ'&Vs&HH1&HH2); rewrite lookup_insert in HH1; simplify_eq.
+      iMod (IH with "[$GCχauth $GCσMLv $GCζauth $GC_per_loc]") as "(GCχauth&GCσMLv&GCζauth&GC_per_loc)"; try done.
+      * intros γ'; destruct (Hbl2 γ') as [HblL HblR]; split.
+        -- intros Hg; destruct (HblL Hg) as (ℓ'&Vs&HH1&HH2). repeat eexists; try done.
+           rewrite lookup_insert_ne in HH1; try done. intros ->; eapply not_elem_of_dom in Hnin; done.
+        -- intros (ℓ'&Vs'&HH1&HH2).
+           assert (γ ≠ γ') as Hnee.
+           1: eapply lookup_union_Some_raw in HH1 as [HH1|(HHr&HH1)]; intros ->; simplify_eq.
+           eapply HblR; repeat eexists; try done. by rewrite lookup_insert_ne.
+      * apply map_subseteq_spec. intros γ' v1 Hv1. eapply lookup_weaken. 2: exact Hsub.
+        rewrite lookup_insert_ne; try done. intros ->; simplify_eq.
+      * iModIntro. iFrame. rewrite lloc_map_pubs_insert_pub. iApply big_sepM_insert.
+        1: apply lloc_map_pubs_lookup_None; left; eapply lookup_union_None_2; done. iFrame.
+        iExists nil, TagDefault, nil. iRight. iRight. iLeft. iPureIntro; split; first done.
+        apply lookup_union_None_2; try done. eapply not_elem_of_dom. intros H%Hother_blocks.
+        by eapply not_elem_of_dom in Hnold.
+  - rewrite -insert_union_r in Hbl2|-*; last done.
+    rewrite lloc_map_pubs_insert_foreign -lloc_map_pubs_delete delete_notin; last by apply lookup_union_None_2.
+    iApply (IH); try done.
+    + intros γ'; destruct (Hbl2 γ') as [HblL HblR]; split.
+      * intros Hg; destruct (HblL Hg) as (ℓ'&Vs&[(_&HH1)|(HH1L&HH1R)]%lookup_insert_Some&HH2); first simplify_eq.
+        by repeat eexists.
+      * intros (ℓ'&Vs&HH1&HH2).
+        assert (γ ≠ γ') as Hnee.
+        1: eapply lookup_union_Some_raw in HH1 as [HH1|(HHr&HH1)]; intros ->; simplify_eq.
+        eapply HblR; repeat eexists; try done. by rewrite lookup_insert_ne.
+    + apply map_subseteq_spec. intros γ' v1 Hv1. eapply lookup_weaken. 2: exact Hsub.
+      rewrite lookup_insert_ne; try done. intros ->; simplify_eq.
+    + iFrame.
+  - rewrite -insert_union_r in Hbl2|-*; last done.
+    rewrite lloc_map_pubs_insert_priv -lloc_map_pubs_delete delete_notin; last by apply lookup_union_None_2.
+    iApply (IH); try done.
+    + intros γ'; destruct (Hbl2 γ') as [HblL HblR]; split.
+      * intros Hg; destruct (HblL Hg) as (ℓ'&Vs&[(_&HH1)|(HH1L&HH1R)]%lookup_insert_Some&HH2); first simplify_eq.
+        by repeat eexists.
+      * intros (ℓ'&Vs&HH1&HH2).
+        assert (γ ≠ γ') as Hnee.
+        1: eapply lookup_union_Some_raw in HH1 as [HH1|(HHr&HH1)]; intros ->; simplify_eq.
+        eapply HblR; repeat eexists; try done. by rewrite lookup_insert_ne.
+    + apply map_subseteq_spec. intros γ' v1 Hv1. eapply lookup_weaken. 2: exact Hsub.
+      rewrite lookup_insert_ne; try done. intros ->; simplify_eq.
+    + iFrame.
+Qed.
+
+(* Final step: Integrate the ζimm *)
+Lemma GC_SI_to_ML σMLvirt ζvirt ζσ ζnewimm χold χnew :
+    ⌜ζvirt ##ₘ ζnewimm⌝ ∗ ⌜ζσ ##ₘ ζnewimm⌝ ∗ ⌜ζvirt ##ₘ ζσ⌝
+  ∗ ⌜is_store_blocks χnew σMLvirt ζσ⌝
+  ∗ ⌜lloc_map_mono χold χnew⌝
+  ∗ ⌜is_private_blocks χnew ζnewimm⌝ ∗ ⌜is_store χnew (ζσ ∪ (ζvirt ∪ ζnewimm)) σMLvirt⌝ ∗ ⌜dom ζvirt ⊆ dom χold⌝
+  ∗ lloc_own_auth χnew
+  ∗ state_interp (σMLvirt : language.language.state ML_lang)
+  ∗ lstore_own_auth (ζvirt ∪ ζnewimm)
+  ∗ ([∗ map] γ↦ℓ ∈ lloc_map_pubs χold, per_location_invariant_ML ζvirt γ ℓ)
+ ⊢ |==> lstore_own_auth (ζσ ∪ (ζvirt ∪ ζnewimm))
+  ∗ ([∗ map] γ↦ℓ ∈ lloc_map_pubs χnew, per_location_invariant (ζσ ∪ (ζvirt ∪ ζnewimm)) σMLvirt γ ℓ)
+  ∗ lloc_own_auth χnew
+  ∗ state_interp (σMLvirt : language.language.state ML_lang).
+Proof.
+  iIntros "(%Hdisj1&%Hdisj2&%Hdisj3&%Hbl&%Hmono&%Hpriv&%Hisstore&%Hother_blocks&GCχauth&GCζauth&GCσMLv&GC_per_loc)".
+  iMod (GC_SI_to_ML_2 with "[$GCχauth $GCζauth $GCσMLv $GC_per_loc]") as "(GCχauth&GCζauth&GCσMLv&GC_per_loc)".
+  1: iPureIntro; split_and!; try done.
+  iFrame.
+  iModIntro.
+  clear Hbl Hmono Hisstore Hother_blocks χold.
+  rewrite map_union_assoc.
+  iStopProof.
+  induction ζnewimm as [|γ blk ζnewimm Hnone IH] using map_ind;
+  iIntros "GC_per_loc".
+  1: by rewrite map_union_empty.
+  apply map_disjoint_insert_r in Hdisj1 as [Hd1 Hdisj1].
+  apply map_disjoint_insert_r in Hdisj2 as [Hd2 Hdisj2].
+  iPoseProof (IH with "GC_per_loc") as "GC_per_loc"; try done.
+  - intros γ' Hdom. eapply Hpriv. rewrite dom_insert_L. set_solver.
+  - rewrite -insert_union_r.
+    + iApply GC_per_loc_modify_ζ; last done.
+      apply lloc_map_pubs_lookup_None. right. left.
+      eapply Hpriv. by rewrite dom_insert_L; set_solver.
+    + by eapply lookup_union_None_2.
 Qed.
 
 Lemma wrap_interp_ml_to_c vs ρml σ ws ρc mem :
@@ -82,45 +660,43 @@ Proof using.
                     Hstore & Hvals & ? & ? & ? & Hroots & ?).
 
   iNamed "Hst". iNamed "SIML". iNamed "SIGCrem".
-  iDestruct (ghost_var_split _ _ (1/2) (1/2) with "[SIinit]") as "[SIinit GCinit]".
-  { rewrite {1}(_: 1 = 1/2+1/2)%Qp // Qp.half_half //. }
+  iNamed "HSI_block_level". iNamed "HSI_GC". SI_GC_agree.
   iMod (ghost_var_update_halves with "Hb SIbound") as "(Hnb & SIbound)".
   iMod (ghost_var_update_halves with "SIζ GCζ") as "(SIζ & GCζ)".
   iMod (ghost_var_update_halves with "SIχ GCχ") as "(SIχ & GCχ)".
   iMod (ghost_var_update_halves with "SIθ GCθ") as "(SIθ & GCθ)".
   iMod (ghost_var_update_halves with "SIroots GCroots") as "(SIroots & GCroots)".
   apply map_disjoint_union_r in Hζdisj as [Hζdisj1 Hζdisj2].
-  iMod (lstore_own_insert_many with "SIζvirt") as "(SIζvirt & SIζnewimm)"; first done.
-  iMod (lloc_own_mono with "SIAχ") as "SIAχ"; first done.
+  iMod (lstore_own_insert_many with "GCζauth") as "(GCζauth & SIζnewimm)"; first done.
+  iMod (lloc_own_mono with "GCχauth") as "GCχauth"; first done.
   assert (ζσ ##ₘ ζnewimm) as Hdisj2 by by eapply is_store_blocks_is_private_blocks_disjoint.
   assert (ζC ρc = ζσ ∪ (ζML ρml ∪ ζnewimm)) as H6B.
   1: { rewrite map_union_assoc. rewrite (map_union_comm ζσ); first done. by symmetry. }
-  iPoseProof (block_sim_arr_of_auth _ _ _ _ _ vs lvs with "SIAχ SIζvirt") as "#Hsim".
+  iPoseProof (block_sim_arr_of_auth _ _ _ _ _ vs lvs with "GCχauth GCζauth") as "#Hsim".
   5: eassumption. 1-3:done. 1: by apply map_disjoint_union_r.
+  iPoseProof (big_sepM_dom with "GCrootspto") as "GCrootspto".
   iMod (set_to_some with "HσCv GCrootspto") as "(HσCv & GCrootspto)"; first done.
-
+  iMod (GC_SI_to_ML with "[$GCζauth $GCχNone $GCχauth $HσML]") as "(GCζauth&GC_per_loc&GCχauth&GCσMLv)".
+  1: (iPureIntro; split_and!; try done).
+  1: by rewrite -H6B.
   iModIntro. iFrame "Hnb". rewrite /= /named.
   iFrame "HσCv SIζ SIχ SIθ SIroots SIbound".
   iSplitL "SIinit". { iExists false. iFrame. }
   iSplit.
-  { rewrite /GC /named.
-    iExists (ζC ρc), (ζC ρc), ζσ, (ζML ρml ∪ ζnewimm).
-    iExists (χC ρc), (χC ρc), σ, (rootsC ρc), (rootsML ρml).
-    iFrame. iSplit.
-    { rewrite pub_locs_in_lstore_insert_priv_store; last done.
-      erewrite pub_locs_in_lstore_mono at 1; [| eauto..]; [].
-      iFrame "SIAχNone". }
-    iPureIntro; split_and!; eauto.
-    { reflexivity. }
-    { by apply map_disjoint_union_r. }
-    { rewrite dom_union_L. apply union_least.
-      - etransitivity; [ eapply Hother_blocks |].
-        eapply subseteq_dom, Hmono.
-      - eapply elem_of_subseteq. intros γ Hγ.
-        by eapply elem_of_dom_2, Hprivblocks. }
-    { split; first done. split; first apply Hmono.
-      intros γ v1 v2 HH1 HH2. simplify_map_eq. econstructor. } }
-  { iExists _; by iFrame "Hsim". }
+  { rewrite /GC /SI_block_level /SI_GC /named.
+    iExists (ζC ρc), (ζC ρc), (χC ρc), (χC ρc), (rootsC ρc). iFrame.
+    iSplitR "GCrootsm GCrootspto"; last first.
+    { iSplit; first (iExists _; iFrame); iPureIntro; split_and!; try done.
+      eapply expose_llocs_refl, Hmono. }
+    { iExists σ. rewrite !H6B. iFrame.
+      iPureIntro. split; try apply Hblocks.
+      rewrite !dom_union_L. repeat apply union_least;
+      intros γ Hγ.
+      - destruct Hblocks as [Hb1 Hb2]. apply Hb2 in Hγ as (ℓ&Vs&HH1&HH2).
+        eapply elem_of_dom_2; done.
+      - edestruct Hmono as [Hm1 Hm2]. eapply subseteq_dom; first exact Hm1. by apply Hother_blocks.
+      - by eapply elem_of_dom_2, Hprivblocks. } }
+  iExists _; iFrame "Hsim". done.
 Qed.
 
 End BoundaryLaws.
